Big Catch up

src/updated/src/SubstSemantics.v
@@ -3,7 +3,6 @@ Require Export Exceptions.
 Require Export Auxiliaries.
 
 Import ListNotations.
-Import Auxiliaries.
 
 Definition lit_eqb (l1 l2 : Literal) : bool :=
 match l1, l2 with
@@ -101,39 +100,6 @@ match p with
               end
 end.
 
-Compute (match_pattern (PTuple []) (VTuple []) ).
-Compute (match_pattern (PTuple [PNil]) (VTuple [VNil]) ).
-Compute (match_pattern (PTuple [PNil]) (VTuple [VVar 1]) ).
-Compute (match_pattern (PTuple [PVar]) (VTuple [VNil]) ).
-Compute (match_pattern (PTuple [PVar]) (VTuple [VVar 1]) ).
-Compute (match_pattern (PTuple [PVar; PNil]) (VTuple [VVar 1; VNil]) ).
-Compute (match_pattern (PTuple [PVar; PVar]) (VTuple [VVar 1; VVar 2]) ).
-Compute (match_pattern (PTuple [PVar; PVar]) (VTuple [VVar 1; VNil]) ).
-Compute (match_pattern (PTuple [PVar; PNil]) (VTuple [VVar 1; VVar 2]) ).
-Compute (match_pattern (PTuple [PNil; PVar]) (VTuple [VVar 1; VVar 2]) ).
-Compute (match_pattern (PTuple [PNil; PVar]) (VTuple [VNil; VVar 2]) ).
-
-Compute (match_pattern (PMap [])            (VMap []) ).
-Compute (match_pattern (PMap [(PNil,PNil)]) (VMap [(VNil,VNil)]) ).
-
-Compute (match_pattern (PMap [(PVar,PNil)]) (VMap [(VNil,VNil)]) ).
-Compute (match_pattern (PMap [(PNil,PVar)]) (VMap [(VNil,VNil)]) ).
-Compute (match_pattern (PMap [(PNil,PNil)]) (VMap [(VVar 1,VNil)]) ).
-Compute (match_pattern (PMap [(PNil,PNil)]) (VMap [(VNil,VVar 2)]) ).
-
-Compute (match_pattern (PMap [(PVar,PVar)]) (VMap [(VNil,VNil)]) ).
-Compute (match_pattern (PMap [(PVar,PNil)]) (VMap [(VVar 1,VNil)]) ).
-Compute (match_pattern (PMap [(PVar,PNil)]) (VMap [(VNil,VVar 2)]) ).
-Compute (match_pattern (PMap [(PNil,PVar)]) (VMap [(VVar 1,VNil)]) ).
-Compute (match_pattern (PMap [(PNil,PVar)]) (VMap [(VNil,VVar 2)]) ).
-Compute (match_pattern (PMap [(PNil,PNil)]) (VMap [(VVar 1,VVar 2)]) ).
-
-Compute (match_pattern (PMap [(PVar,PVar)]) (VMap [(VVar 1,VNil)]) ).
-Compute (match_pattern (PMap [(PVar,PVar)]) (VMap [(VNil,VVar 2)]) ).
-Compute (match_pattern (PMap [(PVar,PNil)]) (VMap [(VVar 1,VVar 2)]) ).
-Compute (match_pattern (PMap [(PNil,PVar)]) (VMap [(VVar 1,VVar 2)]) ).
-Compute (match_pattern (PMap [(PVar,PVar)]) (VMap [(VVar 1,VVar 2)]) ).
-
 Fixpoint match_pattern_list (pl : list Pattern) (vl : list ValueExpression) : option (list ValueExpression) :=
 match pl,vl with
   | (p::ps), (v::vs) => match match_pattern p v with
@@ -152,17 +118,25 @@ Definition convert_to_closlist (l : list (nat * nat * Expression)) : (list Value
 map (fun '(id,vc,e) => (VClos l id vc e)) l.
 
 
-(* TODO (ValueSequence + Exception) -> Prog Result *)
-
 Inductive ProgResult : Type :=
-| Expression (e : Expression) (* RExp *)
-| ValueSequence (vs : list ValueExpression) (* RValSeq *)
-| Exception (e : Exception) (* RExc *)
+| ExpRes (e : Expression) (* RExp *) (* Expression *)
+| ValSeqRes (vs : list ValueExpression) (* RValSeq *) (* ValueSequence *)
+| ExcRes (e : Exception) (* RExc *) (* Exception *)
 .
 
+Reserved Notation "'PROG' Γ ⊢ e" (at level 69, no associativity).
+Inductive ProgResultScope : ProgResult -> nat -> Prop :=
+| expScope Γ e : EXP Γ ⊢ e -> PROG Γ ⊢ (ExpRes e)
+| excScope Γ class reason details : VAL Γ ⊢ reason -> VAL Γ ⊢ details
+                                    -> PROG Γ ⊢ (ExcRes (class,reason,details))
+| valSeqScope Γ vl : (forall i, i < (length vl) -> VAL Γ ⊢ (nth i vl (VNil))) -> PROG Γ ⊢ (ValSeqRes vl)
+where "'PROG' Γ ⊢ e" := (ProgResultScope e Γ).
 
-Definition list_subst (l : list ValueExpression) (ξ : Substitution) : Substitution :=
-  fold_right (fun v acc => v .: acc) ξ l.
+Notation "'PROGCLOSED' v" := (PROG 0 ⊢ v) (at level 5).
+
+
+(* Definition list_subst (l : list ValueExpression) (ξ : Substitution) : Substitution :=
+  fold_right (fun v acc => v .: acc) ξ l. *)
 
 Reserved Notation "⟨ fs , e ⟩ --> ⟨ fs' , e' ⟩" (at level 50).
 
@@ -172,58 +146,58 @@ Inductive step : FrameStack -> ProgResult -> FrameStack -> ProgResult -> Prop :=
 (** Value Expressions**)
 (**  Cooling *)
 | cool_value v xs:
-  ⟨ xs, Expression (Val v) ⟩ --> ⟨ xs, ValueSequence [v] ⟩
+  ⟨ xs, ExpRes (Val v) ⟩ --> ⟨ xs, ValSeqRes [v] ⟩
 
 
 (**  Values *)
 (**  Cooling *)
 | cool_Values_empty xs :
-  ⟨ xs, Expression (Exp (EValues [])) ⟩ --> ⟨ xs, ValueSequence [] ⟩
+  ⟨ xs, ExpRes (Exp (EValues [])) ⟩ --> ⟨ xs, ValSeqRes [] ⟩
 | cool_Values_1 vl e el v xs :
-  ⟨ (FValues vl (e::el))::xs, ValueSequence [v]⟩ --> ⟨ (FValues (vl++[v]) el)::xs, Expression e ⟩
+  ⟨ (FValues vl (e::el))::xs, ValSeqRes [v]⟩ --> ⟨ (FValues (vl++[v]) el)::xs, ExpRes e ⟩
 | cool_Values_2 vl v xs :
-  ⟨ (FValues vl [])::xs, ValueSequence [v] ⟩ --> ⟨ xs, ValueSequence (vl++[v]) ⟩
+  ⟨ (FValues vl [])::xs, ValSeqRes [v] ⟩ --> ⟨ xs, ValSeqRes (vl++[v]) ⟩
 (**  Heating *)
 | heat_Values e el xs:
-  ⟨ xs, Expression (Exp (EValues (e::el))) ⟩ --> ⟨ (FValues [] el)::xs, Expression e ⟩
+  ⟨ xs, ExpRes (Exp (EValues (e::el))) ⟩ --> ⟨ (FValues [] el)::xs, ExpRes e ⟩
 
 
 (**  Cons *)
 (**  Cooling *)
 | cool_Cons_1 hd tl xs :
-  ⟨ (FCons1 hd)::xs, ValueSequence [tl] ⟩ --> ⟨ (FCons2 tl)::xs, Expression hd ⟩
+  ⟨ (FCons1 hd)::xs, ValSeqRes [tl] ⟩ --> ⟨ (FCons2 tl)::xs, ExpRes hd ⟩
 | cool_Cons_2 hd tl xs :
-  ⟨ (FCons2 tl)::xs, ValueSequence [hd] ⟩ --> ⟨ xs, ValueSequence [VCons hd tl] ⟩
+  ⟨ (FCons2 tl)::xs, ValSeqRes [hd] ⟩ --> ⟨ xs, ValSeqRes [VCons hd tl] ⟩
 (**  Heating *)
 | heat_Cons hd tl xs :
-  ⟨ xs, Expression (Exp (ECons hd tl)) ⟩ --> ⟨ (FCons1 hd)::xs, Expression tl ⟩
+  ⟨ xs, ExpRes (Exp (ECons hd tl)) ⟩ --> ⟨ (FCons1 hd)::xs, ExpRes tl ⟩
 
 (**  Tuple *)
 (**  Cooling *)
 | cool_Tuple_empty xs :
-  ⟨ xs, Expression (Exp (ETuple [])) ⟩ --> ⟨ xs, ValueSequence [ VTuple [] ] ⟩
+  ⟨ xs, ExpRes (Exp (ETuple [])) ⟩ --> ⟨ xs, ValSeqRes [ VTuple [] ] ⟩
 | cool_Tuple_1 vl e el v xs :
-  ⟨ (FTuple vl (e::el))::xs, ValueSequence [v] ⟩ --> ⟨ (FTuple (vl++[v]) el)::xs, Expression e ⟩
+  ⟨ (FTuple vl (e::el))::xs, ValSeqRes [v] ⟩ --> ⟨ (FTuple (vl++[v]) el)::xs, ExpRes e ⟩
 | cool_Tuple_2 vl v xs :
-  ⟨ (FTuple vl [])::xs, ValueSequence [v] ⟩ --> ⟨ xs, ValueSequence [ VTuple (vl++[v]) ] ⟩
+  ⟨ (FTuple vl [])::xs, ValSeqRes [v] ⟩ --> ⟨ xs, ValSeqRes [ VTuple (vl++[v]) ] ⟩
 (**  Heating *)
 | heat_Tuple e el xs:
-  ⟨ xs, Expression (Exp (ETuple (e::el))) ⟩ --> ⟨ (FTuple [] el)::xs, Expression e ⟩
+  ⟨ xs, ExpRes (Exp (ETuple (e::el))) ⟩ --> ⟨ (FTuple [] el)::xs, ExpRes e ⟩
 
 
 (**  Map *)
 (**  Cooling *)
 | cool_Map_empty xs :
-  ⟨ xs, Expression (Exp (EMap [])) ⟩ --> ⟨ xs, ValueSequence [ VMap [] ] ⟩
+  ⟨ xs, ExpRes (Exp (EMap [])) ⟩ --> ⟨ xs, ValSeqRes [ VMap [] ] ⟩
 | cool_Map_1  vl sn fs el xs :
-  ⟨ (FMap1 vl sn el)::xs, ValueSequence [fs] ⟩ --> ⟨ (FMap2 vl fs el)::xs, Expression sn ⟩
+  ⟨ (FMap1 vl sn el)::xs, ValSeqRes [fs] ⟩ --> ⟨ (FMap2 vl fs el)::xs, ExpRes sn ⟩
 | cool_Map_2  vl fs sn fs' sn' el xs :
-  ⟨ (FMap2 vl fs ((fs',sn')::el))::xs, ValueSequence [sn] ⟩ --> ⟨ (FMap1 (vl++[(fs,sn)]) sn' el)::xs, Expression fs' ⟩
+  ⟨ (FMap2 vl fs ((fs',sn')::el))::xs, ValSeqRes [sn] ⟩ --> ⟨ (FMap1 (vl++[(fs,sn)]) sn' el)::xs, ExpRes fs' ⟩
 | cool_Map_3  vl fs sn xs :
-  ⟨ (FMap2 vl fs [])::xs, ValueSequence [sn] ⟩ --> ⟨ xs, ValueSequence [ VMap (vl++[(fs,sn)]) ] ⟩
+  ⟨ (FMap2 vl fs [])::xs, ValSeqRes [sn] ⟩ --> ⟨ xs, ValSeqRes [ VMap (vl++[(fs,sn)]) ] ⟩
 (**  Heating *)
 | heat_Map fs sn el xs :
-  ⟨ xs, Expression (Exp (EMap ((fs,sn)::el))) ⟩ --> ⟨ (FMap1 [] sn el)::xs, Expression fs ⟩
+  ⟨ xs, ExpRes (Exp (EMap ((fs,sn)::el))) ⟩ --> ⟨ (FMap1 [] sn el)::xs, ExpRes fs ⟩
 
 
 (**  PrimOp *) (*TODO: Auxiliaries *) (* "inl res" is a ValueExpression*)
@@ -231,94 +205,98 @@ Inductive step : FrameStack -> ProgResult -> FrameStack -> ProgResult -> Prop :=
 (**  Cooling *)
 | cool_PrimOp_empty f xs res eff :
   eval f [] [] = (inl res, eff) ->
-  ⟨ xs, Expression(Exp (EPrimOp f [])) ⟩ --> ⟨ xs, ValueSequence res ⟩
+  ⟨ xs, ExpRes (Exp (EPrimOp f [])) ⟩ --> ⟨ xs, ValSeqRes res ⟩
 | cool_PrimOp_1 f vl e el v xs :
-  ⟨ (FPrimOp f vl (e::el))::xs, ValueSequence [v] ⟩ --> ⟨ (FPrimOp f (vl++[v]) el)::xs, Expression e ⟩
+  ⟨ (FPrimOp f vl (e::el))::xs, ValSeqRes [v] ⟩ --> ⟨ (FPrimOp f (vl++[v]) el)::xs, ExpRes e ⟩
 | cool_PrimOp_2 f vl v xs res eff :
   eval f (vl++[v]) [] = (inl res, eff) ->
-  ⟨ (FPrimOp f vl [])::xs, ValueSequence [v] ⟩ --> ⟨ xs, ValueSequence res ⟩
+  ⟨ (FPrimOp f vl [])::xs, ValSeqRes [v] ⟩ --> ⟨ xs, ValSeqRes res ⟩
 (**  Heating *)
 | heat_PrimOp f e el xs :
-  ⟨ xs, Expression (Exp (EPrimOp f (e::el))) ⟩ --> ⟨ (FPrimOp f [] el)::xs, Expression e ⟩
+  ⟨ xs, ExpRes (Exp (EPrimOp f (e::el))) ⟩ --> ⟨ (FPrimOp f [] el)::xs, ExpRes e ⟩
 (** Exceptions *)
 | err_PrimOp_1 f xs exc eff : (* in this case there were no parameters to evaluate *)
   eval f [] [] = (inr exc, eff) ->
-  ⟨ xs, Expression(Exp (EPrimOp f [])) ⟩ --> ⟨ xs, Exception exc ⟩
+  ⟨ xs, ExpRes (Exp (EPrimOp f [])) ⟩ --> ⟨ xs, ExcRes exc ⟩
 | err_PrimOp_2 f vl v xs exc eff : (* there were parameters *)
   eval f (vl++[v]) [] = (inr exc, eff) ->
-  ⟨ (FPrimOp f vl [])::xs, ValueSequence [v] ⟩ --> ⟨ xs, Exception exc ⟩
+  ⟨ (FPrimOp f vl [])::xs, ValSeqRes [v] ⟩ --> ⟨ xs, ExcRes exc ⟩
 
 (**  Let *)
 (**  Cooling *)
 | cool_Let l e2 vs xs :
   length vs = l ->
-  ⟨ (FLet l e2)::xs, ValueSequence vs ⟩ --> ⟨ xs, Expression (e2.[ list_subst vs idsubst ]) ⟩ (* TODO: e2.[ ? ] *)
+  ⟨ (FLet l e2)::xs, ValSeqRes vs ⟩ --> ⟨ xs, ExpRes (e2.[ list_subst vs idsubst ]) ⟩
 (**  Heating *)
 | heat_Let l e1 e2 xs :
-  ⟨ xs, Expression(Exp (ELet l e1 e2)) ⟩ --> ⟨ (FLet l e2)::xs, Expression e1 ⟩
+  ⟨ xs, ExpRes (Exp (ELet l e1 e2)) ⟩ --> ⟨ (FLet l e2)::xs, ExpRes e1 ⟩
 
 
 (**  Seq *)
 (**  Cooling *)
 | cool_Seq e2 v xs :
-  ⟨ (FSeq e2)::xs, ValueSequence [v] ⟩ --> ⟨ xs, Expression e2 ⟩
+  ⟨ (FSeq e2)::xs, ValSeqRes [v] ⟩ --> ⟨ xs, ExpRes e2 ⟩
 (**  Heating *)
 | heat_Seq e1 e2 xs :
-  ⟨ xs, Expression (Exp (ESeq e1 e2)) ⟩ --> ⟨ (FSeq e2)::xs, Expression e1 ⟩
-  
+  ⟨ xs, ExpRes (Exp (ESeq e1 e2)) ⟩ --> ⟨ (FSeq e2)::xs, ExpRes e1 ⟩
+
+
 (**  Fun *)
 (**  Cooling *)
 | cool_fun e vl xs :
-  ⟨ xs, Expression (Exp (EFun vl e)) ⟩ --> ⟨ xs, ValueSequence [ VClos [] 0 vl e ] ⟩ (*TODO : id not 0*)
+  ⟨ xs, ExpRes (Exp (EFun vl e)) ⟩ --> ⟨ xs, ValSeqRes [ VClos [] 0 vl e ] ⟩ (*TODO : id not 0*)
 
 
-(**  Call *) (*TODO : will be the same as PrimOp, use the eval from the Auxilieries*)
+(**  Call *)
 (**  Cooling *)
 | cool_Call_empty f xs res eff :
   eval f [] [] = (inl res, eff) ->
-  ⟨ xs, Expression (Exp (ECall f [])) ⟩ --> ⟨ xs, ValueSequence res ⟩
+  ⟨ xs, ExpRes (Exp (ECall f [])) ⟩ --> ⟨ xs, ValSeqRes res ⟩
 | cool_Call_1 f vl e el v xs :
-  ⟨ (FCall f vl (e::el))::xs, ValueSequence [v] ⟩ --> ⟨ (FCall f (vl++[v]) el)::xs, Expression e ⟩
+  ⟨ (FCall f vl (e::el))::xs, ValSeqRes [v] ⟩ --> ⟨ (FCall f (vl++[v]) el)::xs, ExpRes e ⟩
 | cool_Call_2 f vl v xs res eff :
   eval f (vl++[v]) [] = (inl res, eff) ->
-  ⟨ (FCall f vl [])::xs, ValueSequence [v] ⟩ --> ⟨ xs, ValueSequence res ⟩
+  ⟨ (FCall f vl [])::xs, ValSeqRes [v] ⟩ --> ⟨ xs, ValSeqRes res ⟩
 (**  Heating *)
 | heat_Call f e el xs :
-  ⟨ xs, Expression (Exp (ECall f (e::el))) ⟩ --> ⟨ (FCall f [] el)::xs, Expression e ⟩
+  ⟨ xs, ExpRes (Exp (ECall f (e::el))) ⟩ --> ⟨ (FCall f [] el)::xs, ExpRes e ⟩
 (** Exceptions *)
 | err_Call_1 f exc eff xs : (* in this case there were no parameters to evaluate *)
   eval f [] [] = (inr exc, eff) ->
-  ⟨ xs, Expression (Exp (ECall f [])) ⟩ --> ⟨ xs, Exception exc ⟩
+  ⟨ xs, ExpRes (Exp (ECall f [])) ⟩ --> ⟨ xs, ExcRes exc ⟩
 | err_Call_2 f v vl exc eff xs : (* there were parameters *)
   eval f (vl++[v]) [] = (inr exc, eff) ->
-  ⟨ (FCall f vl [])::xs, ValueSequence [v] ⟩ --> ⟨ xs, Exception exc ⟩
+  ⟨ (FCall f vl [])::xs, ValSeqRes [v] ⟩ --> ⟨ xs, ExcRes exc ⟩
 
 (**  App *) (* On paper *) (* in "EApp e el" e needs to evaluate to a VClos but it will only be checked when el is done *)
-(**  Cooling *) (*TODO: empty FApp1 *) (* TODO: vc = length vl, when to evaluate? *)
+(**  Cooling *) (*TODO: empty FApp1 *)
 | cool_App_empty vl' ext id e xs :
   convert_to_closlist ext = vl' ->
-  ⟨ (FApp1 [])::xs, ValueSequence [(VClos ext id 0 e)] ⟩ --> ⟨ xs, Expression e.[list_subst (vl') idsubst] ⟩
+  ⟨ (FApp1 [])::xs, ValSeqRes [(VClos ext id 0 e)] ⟩ --> ⟨ xs, ExpRes e.[list_subst (vl') idsubst] ⟩
 | cool_App_1 e el v xs :
-  ⟨ (FApp1 (e::el))::xs, ValueSequence [v] ⟩ --> ⟨ (FApp2 v [] el)::xs, Expression e ⟩
+  ⟨ (FApp1 (e::el))::xs, ValSeqRes [v] ⟩ --> ⟨ (FApp2 v [] el)::xs, ExpRes e ⟩
 | cool_App_2a v' vl e el v xs :
-  ⟨ (FApp2 v' vl (e::el))::xs, ValueSequence [v] ⟩ --> ⟨ (FApp2 v' (vl++[v]) el)::xs, Expression e ⟩
+  ⟨ (FApp2 v' vl (e::el))::xs, ValSeqRes [v] ⟩ --> ⟨ (FApp2 v' (vl++[v]) el)::xs, ExpRes e ⟩
 | cool_App_2b vl' ext id vc e' vl v xs :
   vc = (length (vl) + 1) ->
   convert_to_closlist ext = vl' ->
-  ⟨ (FApp2 (VClos ext id vc e') vl [])::xs, ValueSequence [v] ⟩ --> ⟨ xs, Expression (e'.[list_subst (vl'++(vl++[v])) idsubst]) ⟩
+  ⟨ (FApp2 (VClos ext id vc e') vl [])::xs, ValSeqRes [v] ⟩ --> ⟨ xs, ExpRes (e'.[list_subst (vl'++(vl++[v])) idsubst]) ⟩
 (**  Heating *)
 | heat_App e el xs :
-  ⟨ xs, Expression (Exp (EApp e el)) ⟩ --> ⟨ (FApp1 el)::xs, Expression e ⟩
+  ⟨ xs, ExpRes (Exp (EApp e el)) ⟩ --> ⟨ (FApp1 el)::xs, ExpRes e ⟩
 (** Exceptions *) (*TODO badarity FApp1 version*)
-| err_App_badariry ext id vc e' vl xs v :
+| err_App_badariry_1 ext id vc e xs :
+  vc <> 0 ->
+  ⟨ (FApp1 [])::xs, ValSeqRes [(VClos ext id vc e)] ⟩ --> ⟨ xs, ExcRes (badarity (VClos ext id vc e)) ⟩
+| err_App_badariry_2 ext id vc e' vl xs v :
   vc <> (length (vl) + 1) ->
-  ⟨ (FApp2 (VClos ext id vc e') vl [])::xs, ValueSequence [v] ⟩ --> ⟨ xs, Exception (badarity (VClos ext id vc e')) ⟩
+  ⟨ (FApp2 (VClos ext id vc e') vl [])::xs, ValSeqRes [v] ⟩ --> ⟨ xs, ExcRes (badarity (VClos ext id vc e')) ⟩
 | err_App_noclos_1 v xs : (* when it had no other expressions to evalate ([] case) *)
   (forall ext id vc e, v <> (VClos ext id vc e)) ->
-  ⟨ (FApp1 [])::xs, ValueSequence [v] ⟩ --> ⟨ xs, Exception (badfun v) ⟩
+  ⟨ (FApp1 [])::xs, ValSeqRes [v] ⟩ --> ⟨ xs, ExcRes (badfun v) ⟩
 | err_App_noclos_2 v' vl v xs : (* when it had expressions to evaluate *)
   (forall ext id vc e', v' <> (VClos ext id vc e')) ->
-  ⟨ (FApp2 v' vl [])::xs, ValueSequence [v] ⟩ --> ⟨ xs, Exception (badfun v') ⟩
+  ⟨ (FApp2 v' vl [])::xs, ValSeqRes [v] ⟩ --> ⟨ xs, ExcRes (badfun v') ⟩
 
 
 (**  Case *)
@@ -326,96 +304,93 @@ Inductive step : FrameStack -> ProgResult -> FrameStack -> ProgResult -> Prop :=
 (* eval started or ongoing, the first pattern matched, e1 the guard needs to be evaluated *)
 | cool_Case_1m lp e1 e2 l vs vs' xs :
   match_pattern_list lp vs = Some vs' ->
-  ⟨ (FCase1 ((lp,e1,e2)::l))::xs, ValueSequence vs ⟩ --> ⟨ (FCase2 vs lp e2 l vs')::xs, Expression (e1.[list_subst (vs') idsubst]) ⟩
+  ⟨ (FCase1 ((lp,e1,e2)::l))::xs, ValSeqRes vs ⟩ --> ⟨ (FCase2 vs lp e2 l vs')::xs, ExpRes (e1.[list_subst (vs') idsubst]) ⟩
 (* eval started or ongoing, the first pattern doesn't match, so case jumps to the next option where the pattern needs to match first. *)
 | cool_Case_1nm lp e1 e2 l vs xs :
   match_pattern_list lp vs = None ->
-  ⟨ (FCase1 ((lp,e1,e2)::l))::xs, ValueSequence vs ⟩ --> ⟨ (FCase1 l)::xs, ValueSequence vs ⟩
+  ⟨ (FCase1 ((lp,e1,e2)::l))::xs, ValSeqRes vs ⟩ --> ⟨ (FCase1 l)::xs, ValSeqRes vs ⟩
 (* eval ongoing, the last pattern matched, the guard is true, so case ends*)
 | cool_Case_2mt vs lp e' l vs' xs :
-  ⟨ (FCase2 vs lp e' l vs')::xs, ValueSequence [ VLit (Atom "true") ] ⟩ --> ⟨ xs, Expression (e'.[list_subst (vs') idsubst]) ⟩
+  ⟨ (FCase2 vs lp e' l vs')::xs, ValSeqRes [ VLit (Atom "true") ] ⟩ --> ⟨ xs, ExpRes (e'.[list_subst (vs') idsubst]) ⟩
 (* eval ongoing, the last pattern matched, the guard is false, so case jumps to the next option where the pattern needs to match first. *)
 | cool_Case_2mf vs lp' e' l vs' xs :
-  ⟨ (FCase2 vs lp' e' l vs')::xs, ValueSequence [ VLit (Atom "false") ] ⟩ --> ⟨ (FCase1 l)::xs, ValueSequence vs ⟩
+  ⟨ (FCase2 vs lp' e' l vs')::xs, ValSeqRes [ VLit (Atom "false") ] ⟩ --> ⟨ (FCase1 l)::xs, ValSeqRes vs ⟩
 (**  Heating *)
 | heat_Case e l xs:
-  ⟨ xs, Expression (Exp (ECase e l)) ⟩ --> ⟨ (FCase1 l)::xs, Expression e ⟩
+  ⟨ xs, ExpRes (Exp (ECase e l)) ⟩ --> ⟨ (FCase1 l)::xs, ExpRes e ⟩
 (** Exceptions *)
 | err_Case_empty vs xs:
-  ⟨ (FCase1 [])::xs, ValueSequence vs ⟩ --> ⟨ xs, Exception if_clause ⟩
+  ⟨ (FCase1 [])::xs, ValSeqRes vs ⟩ --> ⟨ xs, ExcRes if_clause ⟩
 
 (**  LetRec *)
 (**  Cooling *)
 (**  Heating *)
 | heat_LetRec l e lc xs :
   convert_to_closlist (map (fun '(x,y) => (0,x,y)) l) = lc -> (*TODO: for now the funids are 0 coded in *)
-  ⟨ xs, Expression (Exp (ELetRec l e)) ⟩ --> ⟨ xs, Expression e.[list_subst (lc) idsubst] ⟩
+  ⟨ xs, ExpRes (Exp (ELetRec l e)) ⟩ --> ⟨ xs, ExpRes e.[list_subst (lc) idsubst] ⟩
 
 
 (**  Try *)
 (**  Cooling *)
 | cool_Try_ok vl1 e2 vl2 e3 vs xs:
   vl1 = length vs ->
-  ⟨ (FTry vl1 e2 vl2 e3)::xs, ValueSequence vs ⟩ --> ⟨ xs, Expression e2.[ list_subst vs idsubst ] ⟩
+  ⟨ (FTry vl1 e2 vl2 e3)::xs, ValSeqRes vs ⟩ --> ⟨ xs, ExpRes e2.[ list_subst vs idsubst ] ⟩
 | cool_Try_err vl1 e2 e3 class reason details xs:  (* in CErlang exceptions always have 3 part*)
-  ⟨ (FTry vl1 e2 3 e3)::xs, Exception (class, reason, details) ⟩ --> ⟨ xs, Expression e3.[ list_subst [exclass_to_value class; reason; details] idsubst ] ⟩
+  ⟨ (FTry vl1 e2 3 e3)::xs, ExcRes (class, reason, details) ⟩ --> ⟨ xs, ExpRes e3.[ list_subst [exclass_to_value class; reason; details] idsubst ] ⟩
 (**  Heating *)
 | heat_Try e1 vl1 e2 vl2 e3 xs :
-  ⟨ xs, Expression (Exp (ETry e1 vl1 e2 vl2 e3)) ⟩ --> ⟨ (FTry vl1 e2 vl2 e3)::xs, Expression e1 ⟩
+  ⟨ xs, ExpRes (Exp (ETry e1 vl1 e2 vl2 e3)) ⟩ --> ⟨ (FTry vl1 e2 vl2 e3)::xs, ExpRes e1 ⟩
   
 (** Exceptions *)
 (** Propogation *)
-| propogate_Exception frame e xs :
+| propogate_Exception frame exc xs :
   (forall vl1 e2 vl2 e3 , (FTry vl1 e2 vl2 e3) <> frame)->
-  ⟨ (frame)::xs, Exception e ⟩ --> ⟨ xs, Exception e ⟩
+  ⟨ (frame)::xs, ExcRes exc ⟩ --> ⟨ xs, ExcRes exc ⟩
 
 
 where "⟨ fs , e ⟩ --> ⟨ fs' , e' ⟩" := (step fs e fs' e').
 
 
-Theorem semmantics_rules_determinism :
-  forall fs fs1 fs2 e e1 e2,
-  ⟨ fs , e ⟩ --> ⟨ fs1 , e1 ⟩ ->
-  ⟨ fs , e ⟩ --> ⟨ fs2 , e2 ⟩
-  -> (fs1 = fs2 /\ e1 = e2).
-Proof.
-intros. inversion H; subst; inversion H0; auto; subst.
-* rewrite H1 in H4. inversion H4. subst. auto.
-* rewrite H1 in H4. inversion H4.
-* rewrite H1 in H8. inversion H8. subst. auto.
-* rewrite H1 in H8. inversion H8.
-* rewrite H1 in H4. inversion H4.
-* rewrite H1 in H4. inversion H4. subst. auto.
-* rewrite H1 in H8. inversion H8.
-* rewrite H1 in H8. inversion H8. subst. auto.
-* rewrite H1 in H4. inversion H4. subst. auto.
-* rewrite H1 in H4. inversion H4.
-* rewrite H1 in H8. inversion H8. subst. auto.
-* rewrite H1 in H8. inversion H8.
-* rewrite H1 in H4. inversion H4.
-* rewrite H1 in H4. inversion H4. subst. auto.
-* rewrite H1 in H8. inversion H8.
-* rewrite H1 in H8. inversion H8. subst. auto.
-* auto.
-* specialize (H3 ext id 0 e0). congruence.
-* auto.
-* congruence.
-* specialize (H7 ext id (Datatypes.length vl + 1) e'). congruence.
-* congruence.
-* specialize (H8 ext id vc e'). congruence.
-* specialize (H1 ext id 0 e). congruence.
-* specialize (H1 ext id (Datatypes.length vl + 1) e'). congruence.
-* specialize (H1 ext id vc e'). congruence.
-* rewrite H1 in H10. inversion H10. subst. auto.
-* rewrite H1 in H10. inversion H10.
-* rewrite H1 in H10. inversion H10.
-* auto.
-* specialize (H6 vl1 e0 3 e3). congruence.
-* specialize (H1 vl1 e1 3 e3). congruence.
-Qed.
+
+Reserved Notation "⟨ fs , e ⟩ -[ k ]-> ⟨ fs' , e' ⟩" (at level 50).
+Inductive step_rt : FrameStack -> ProgResult -> nat -> FrameStack -> ProgResult -> Prop :=
+| step_refl fs e : ⟨ fs, e ⟩ -[ 0 ]-> ⟨ fs, e ⟩
+| step_trans fs e fs' e' fs'' e'' k:
+  ⟨ fs, e ⟩ --> ⟨ fs', e'⟩ -> ⟨fs', e'⟩ -[ k ]-> ⟨fs'', e''⟩
+  ->
+  ⟨ fs, e ⟩ -[S k]-> ⟨fs'', e''⟩
+where "⟨ fs , e ⟩ -[ k ]-> ⟨ fs' , e' ⟩" := (step_rt fs e k fs' e').
+
+
+
+Definition step_any (fs : FrameStack) (e : ProgResult) (r : ProgResult) : Prop :=
+  (exists k v, r = ValSeqRes v /\ ⟨fs, e⟩ -[k]-> ⟨[], ValSeqRes v⟩)
+  \/
+  (exists k ex, r = ExcRes ex /\ ⟨fs, e⟩ -[k]-> ⟨[], ExcRes ex⟩).
+
+Notation "⟨ fs , e ⟩ -->* v" := (step_any fs e v) (at level 50).
 
 
 
 
+
+(*
+Reserved Notation "⟨ fs , e ⟩ -->* v" (at level 50).
+Inductive step_any : FrameStack -> ProgResult -> ProgResult -> Prop :=
+
+| valseq_res    fs e r k v  :
+  r = ValueSequence v ->
+  ⟨fs, e⟩ -[k]-> ⟨[], ValueSequence v⟩
+  ->
+  ⟨ fs , e ⟩ -->* r
+
+| exception_res fs e r k ex :
+  r = Exception ex ->
+  ⟨fs, e⟩ -[k]-> ⟨[], Exception ex⟩
+  ->
+  ⟨ fs , e ⟩ -->* r
+
+where "⟨ fs , e ⟩ -->* r" := (step_any fs e r).
+*)
 
 
