src/updated/src/CIU.v
@@ -1,0 +1,235 @@
+Require Export Termination.
+
+Import ListNotations.
+
+
+Definition CIU (e1 e2 : Expression) : Prop :=
+  EXPCLOSED e1 /\ EXPCLOSED e2 /\
+  forall F, FSCLOSED F -> | F, ExpRes e1 | ↓ -> | F, ExpRes e2 | ↓.
+
+
+
+Definition CIU_open (Γ : nat) (e1 e2 : Expression) :=
+  forall ξ, SUBSCOPE Γ ⊢ ξ ∷ 0 ->
+  CIU (e1.[ξ]) (e2.[ξ]).
+
+
+Lemma CIU_closed :
+  forall e1 e2,
+  CIU e1 e2 -> EXPCLOSED e1 /\ EXPCLOSED e2.
+Proof.
+  intros. unfold CIU in H. intuition.
+Qed.
+
+
+Lemma CIU_closed_l : forall {e1 e2},
+    CIU e1 e2 ->
+    EXPCLOSED e1.
+Proof.
+  intros.
+  apply CIU_closed in H.
+  intuition.
+Qed.
+
+Global Hint Resolve CIU_closed_l : core.
+
+
+
+Lemma CIU_closed_r : forall {e1 e2},
+    CIU e1 e2 ->
+    EXPCLOSED e2.
+Proof.
+  intros.
+  apply CIU_closed in H.
+  intuition.
+Qed.
+
+Global Hint Resolve CIU_closed_r : core.
+
+
+Check subst_implies_scope_exp.
+Lemma CIU_open_scope : forall {Γ e1 e2},
+    CIU_open Γ e1 e2 ->
+    EXP Γ ⊢ e1 /\ EXP Γ ⊢ e2.
+Proof.
+  intros.
+  unfold CIU_open in H.
+  split.
+  * destruct e1.
+    - constructor. simpl in H. Check subst_implies_scope_val.
+      apply (subst_implies_scope_val _ _ 0). intros.
+      specialize (H ξ H0). inversion H. inversion H1. auto.
+    - constructor. simpl in H.
+      apply (subst_implies_scope_nval _ _ 0). intros.
+      specialize (H ξ H0). inversion H. inversion H1. auto.
+  * destruct e2.
+    - constructor. simpl in H. Check subst_implies_scope_val.
+      apply (subst_implies_scope_val _ _ 0). intros.
+      specialize (H ξ H0). inversion H. destruct H2. inversion H2.
+      auto.
+    - constructor. simpl in H.
+      apply (subst_implies_scope_nval _ _ 0). intros.
+      specialize (H ξ H0). inversion H. destruct H2. inversion H2.
+      auto.
+Qed.
+
+
+Lemma CIU_open_scope_l : forall {Γ e1 e2},
+    CIU_open Γ e1 e2 ->
+    EXP Γ ⊢ e1.
+Proof.
+  intros.
+  apply CIU_open_scope in H.
+  intuition.
+Qed.
+
+
+Global Hint Resolve CIU_open_scope_l : core.
+
+Lemma CIU_open_scope_r : forall {Γ e1 e2},
+    CIU_open Γ e1 e2 ->
+    EXP Γ ⊢ e2.
+Proof.
+  intros.
+  apply CIU_open_scope in H.
+  intuition.
+Qed.
+
+Global Hint Resolve CIU_open_scope_r : core.
+
+
+(*--- ProgRes Ver ---*)
+(* 
+Definition substProg (ξ : Substitution) (base : ProgResult) : ProgResult :=
+match base with
+| ExpRes e      => ExpRes (e.[ξ])
+| ValSeqRes vs  => ValSeqRes (map (fun x => substVal ξ x) vs)
+| ExcRes (class, reason, details) => ExcRes (class, reason.[ξ]ᵥ, details.[ξ]ᵥ)
+end.
+Notation "s .[ σ ]ₚ" := (substProg σ s)
+  (at level 2, σ at level 200, left associativity,
+   format "s .[ σ ]ₚ" ).
+
+
+Definition CIU (p1 p2 : ProgResult) : Prop :=
+  PROGCLOSED p1 /\ PROGCLOSED p2 /\
+  forall F, FSCLOSED F -> | F, p1 | ↓ -> | F, p2 | ↓.
+
+
+
+Definition CIU_open (Γ : nat) (p1 p2 : ProgResult) :=
+  forall ξ, SUBSCOPE Γ ⊢ ξ ∷ 0 ->
+  CIU (p1.[ξ]ₚ) (p2.[ξ]ₚ).
+
+
+
+Lemma CIU_closed :
+  forall p1 p2,
+  CIU p1 p2 -> PROGCLOSED p1 /\ PROGCLOSED p2.
+Proof.
+  intros. unfold CIU in H. intuition.
+Qed.
+
+
+
+Lemma CIU_closed_l : forall {p1 p2},
+    CIU p1 p2 ->
+    PROGCLOSED p1.
+Proof.
+  intros.
+  apply CIU_closed in H.
+  intuition.
+Qed.
+
+Global Hint Resolve CIU_closed_l : core.
+
+
+
+Lemma CIU_closed_r : forall {p1 p2},
+    CIU p1 p2 ->
+    PROGCLOSED p2.
+Proof.
+  intros.
+  apply CIU_closed in H.
+  intuition.
+Qed.
+
+Global Hint Resolve CIU_closed_r : core.
+
+
+
+Check subst_implies_scope_exp.
+Lemma CIU_open_scope : forall {Γ p1 p2},
+    CIU_open Γ p1 p2 ->
+    PROG Γ ⊢ p1 /\ PROG Γ ⊢ p2.
+Proof.
+  intros.
+  unfold CIU_open in H.
+  split.
+  * destruct p1.
+    - constructor. Check subst_implies_scope_exp.
+      eapply (subst_implies_scope_exp _ _ 0).
+      intros. specialize (H ξ H0). inversion H.
+      inversion H1. auto.
+    - constructor. Check subst_implies_scope_val.
+      intros. eapply (subst_implies_scope_val _ _ 0).
+      intros. specialize (H ξ H1). inversion H.
+      inversion H2. rewrite map_length in H5.
+      specialize (H5 i H0).
+      Check map_nth. remember (fun x : ValueExpression => x.[ξ]ᵥ) as F.
+      replace VNil with (F VNil) in H5 by (subst;simpl;auto).
+      rewrite map_nth in H5. subst. auto.
+    - destruct e. destruct p. constructor.
+      + eapply (subst_implies_scope_val _ _ 0).
+        intros. specialize (H ξ H0). inversion H.
+        inversion H1. auto.
+      + eapply (subst_implies_scope_val _ _ 0).
+        intros. specialize (H ξ H0). inversion H.
+        inversion H1. auto.
+  * destruct p2.
+    - constructor. Check subst_implies_scope_exp.
+      eapply (subst_implies_scope_exp _ _ 0).
+      intros. specialize (H ξ H0). inversion H.
+      destruct H2. inversion H2. auto.
+    - constructor. Check subst_implies_scope_val.
+      intros. eapply (subst_implies_scope_val _ _ 0).
+      intros. specialize (H ξ H1). inversion H.
+      destruct H3. inversion H3. rewrite map_length in H6.
+      specialize (H6 i H0).
+      Check map_nth. remember (fun x : ValueExpression => x.[ξ]ᵥ) as F.
+      replace VNil with (F VNil) in H6 by (subst;simpl;auto).
+      rewrite map_nth in H6. subst. auto.
+    - destruct e. destruct p. constructor.
+      + eapply (subst_implies_scope_val _ _ 0).
+        intros. specialize (H ξ H0). inversion H.
+        destruct H2. inversion H2. auto.
+      + eapply (subst_implies_scope_val _ _ 0).
+        intros. specialize (H ξ H0). inversion H.
+        destruct H2. inversion H2. auto.
+Qed.
+
+
+
+Lemma CIU_open_scope_l : forall {Γ p1 p2},
+    CIU_open Γ p1 p2 ->
+    PROG Γ ⊢ p1.
+Proof.
+  intros.
+  apply CIU_open_scope in H.
+  intuition.
+Qed.
+
+
+Global Hint Resolve CIU_open_scope_l : core.
+
+Lemma CIU_open_scope_r : forall {Γ p1 p2},
+    CIU_open Γ p1 p2 ->
+    PROG Γ ⊢ p2.
+Proof.
+  intros.
+  apply CIU_open_scope in H.
+  intuition.
+Qed.
+
+Global Hint Resolve CIU_open_scope_r : core.
+*)
