src/updated/src/CTX.v
@@ -1,0 +1,948 @@
+Require Export CIU.
+
+Import ListNotations.
+
+Definition Adequate (R : nat -> ProgResult -> ProgResult -> Prop) :=
+  forall p1 p2, R 0 p1 p2 -> |[], p1| ↓ -> |[], p2| ↓.
+
+Definition IsReflexive (R : nat -> ProgResult -> ProgResult -> Prop) :=
+  forall Γ p,
+  PROG Γ ⊢ p -> R Γ p p.
+
+
+(*---------------------------- Non Value Expr Comp ------------------------------------------------------*)
+
+Definition CompatibleEFun (R : nat -> ProgResult -> ProgResult -> Prop) :=
+  forall Γ vl vl' e1 e2, vl = vl' ->
+    EXP (vl + Γ) ⊢ e1 -> EXP (vl' + Γ) ⊢ e2 -> 
+    R (vl + Γ) (ExpRes e1) (ExpRes e2) -> (* TODO: S vl or is it just vl? *)
+    R Γ (ExpRes (Exp (EFun vl e1))) (ExpRes (Exp (EFun vl' e2))).
+
+Definition CompatibleEValues (R : nat -> ProgResult -> ProgResult -> Prop) :=
+  forall Γ el el', length el = length el' ->
+    (forall i, i < length el  -> EXP Γ ⊢ (nth i el (Val VNil))) ->
+    (forall i, i < length el' -> EXP Γ ⊢ (nth i el' (Val VNil))) ->
+    (forall i, i < length el  -> 
+    R Γ (ExpRes (nth i el (Val VNil))) (ExpRes (nth i el' (Val VNil)))) ->
+    R Γ (ExpRes (Exp (EValues el))) (ExpRes (Exp (EValues el'))).
+
+Definition CompatibleECons (R : nat -> ProgResult -> ProgResult -> Prop) :=
+  forall Γ e1 e1' e2 e2',
+    EXP Γ ⊢ e1 -> EXP Γ ⊢ e1' -> 
+    EXP Γ ⊢ e2 -> EXP Γ ⊢ e2' ->
+    R Γ (ExpRes e1) (ExpRes e1') -> 
+    R Γ (ExpRes e2) (ExpRes e2') ->
+    R Γ (ExpRes (Exp (ECons e1 e2))) (ExpRes (Exp (ECons e1' e2'))).
+
+Definition CompatibleETuple (R : nat -> ProgResult -> ProgResult -> Prop) :=
+  forall Γ el el', length el = length el' ->
+    (forall i, i < length el  -> EXP Γ ⊢ (nth i el (Val VNil))) ->
+    (forall i, i < length el' -> EXP Γ ⊢ (nth i el' (Val VNil))) ->
+    (forall i, i < length el -> 
+    R Γ (ExpRes (nth i el (Val VNil))) (ExpRes (nth i el' (Val VNil)))) ->
+    R Γ (ExpRes (Exp (ETuple el))) (ExpRes (Exp (ETuple el'))).
+
+Definition CompatibleEMap (R : nat -> ProgResult -> ProgResult -> Prop) :=
+  forall Γ l l', length l = length l' ->
+    (forall i, i < length l  -> EXP Γ ⊢ (nth i (map fst l) (Val VNil))) ->
+    (forall i, i < length l' -> EXP Γ ⊢ (nth i (map fst l') (Val VNil))) ->
+    (forall i, i < length l  -> EXP Γ ⊢ (nth i (map snd l) (Val VNil))) ->
+    (forall i, i < length l' -> EXP Γ ⊢ (nth i (map snd l') (Val VNil))) ->
+    (forall i, i < length l -> 
+    R Γ (ExpRes (nth i (map fst l) (Val VNil))) (ExpRes (nth i (map fst l') (Val VNil)))) ->
+    (forall i, i < length l -> 
+    R Γ (ExpRes (nth i (map snd l) (Val VNil))) (ExpRes (nth i (map snd l') (Val VNil)))) ->
+    R Γ (ExpRes (Exp (EMap l))) (ExpRes (Exp (EMap l'))).
+
+Definition CompatibleECall (R : nat -> ProgResult -> ProgResult -> Prop) :=
+  forall Γ f f' el el', f = f' -> length el = length el' ->
+    (forall i, i < length el  -> EXP Γ ⊢ (nth i el (Val VNil))) ->
+    (forall i, i < length el' -> EXP Γ ⊢ (nth i el' (Val VNil))) ->
+    (forall i, i < length el -> 
+    R Γ (ExpRes (nth i el (Val VNil))) (ExpRes (nth i el' (Val VNil)))) ->
+    R Γ (ExpRes (Exp (ECall f el))) (ExpRes (Exp (ECall f' el'))).
+
+Definition CompatibleEPrimOp (R : nat -> ProgResult -> ProgResult -> Prop) :=
+  forall Γ f f' el el', f = f' -> length el = length el' ->
+    (forall i, i < length el  -> EXP Γ ⊢ (nth i el (Val VNil))) ->
+    (forall i, i < length el' -> EXP Γ ⊢ (nth i el' (Val VNil))) ->
+    (forall i, i < length el -> 
+    R Γ (ExpRes (nth i el (Val VNil))) (ExpRes (nth i el' (Val VNil)))) ->
+    R Γ (ExpRes (Exp (EPrimOp f el))) (ExpRes (Exp (EPrimOp f' el'))).
+
+Definition CompatibleEApp (R : nat -> ProgResult -> ProgResult -> Prop) :=
+  forall Γ e e' el el', length el = length el' ->
+    EXP Γ ⊢ e ->
+    EXP Γ ⊢ e' ->
+    (forall i, i < length el  -> EXP Γ ⊢ (nth i el (Val VNil))) ->
+    (forall i, i < length el' -> EXP Γ ⊢ (nth i el' (Val VNil))) ->
+    R Γ (ExpRes e) (ExpRes e') ->
+    (forall i, i < length el -> 
+    R Γ (ExpRes (nth i el (Val VNil))) (ExpRes (nth i el' (Val VNil)))) ->
+    R Γ (ExpRes (Exp (EApp e el))) (ExpRes (Exp (EApp e' el'))).
+
+Definition CompatibleECase (R : nat -> ProgResult -> ProgResult -> Prop) := (* TODO: l or l' in places? *)
+  forall Γ e e' l l', length l = length l' ->
+    EXP Γ ⊢ e ->
+    EXP Γ ⊢ e' ->
+    (forall i, i < length l -> 
+    EXP ((patternListScope (nth i (map fst (map fst l)) nil)) + Γ) ⊢ (nth i (map snd (map fst l)) (Val VNil))) ->
+    (forall i, i < length l' -> 
+    EXP ((patternListScope (nth i (map fst (map fst l)) nil)) + Γ) ⊢ (nth i (map snd (map fst l')) (Val VNil))) ->
+    (forall i, i < length l -> 
+    EXP ((patternListScope (nth i (map fst (map fst l)) nil)) + Γ) ⊢ (nth i (map snd l) (Val VNil))) ->
+    (forall i, i < length l' -> 
+    EXP ((patternListScope (nth i (map fst (map fst l)) nil)) + Γ) ⊢ (nth i (map snd l') (Val VNil))) ->
+    (forall i, i < length l ->
+    R ((patternListScope (nth i (map fst (map fst l)) nil)) + Γ)
+    (ExpRes (nth i (map snd (map fst l)) (Val VNil))) (ExpRes (nth i (map snd (map fst l')) (Val VNil)))) ->
+    (forall i, i < length l ->
+    R ((patternListScope (nth i (map fst (map fst l)) nil)) + Γ)
+    (ExpRes (nth i (map snd l) (Val VNil))) (ExpRes (nth i (map snd l') (Val VNil)))) ->
+    R Γ (ExpRes (Exp (ECase e l))) (ExpRes (Exp (ECase e' l'))).
+
+Definition CompatibleELet (R : nat -> ProgResult -> ProgResult -> Prop) :=
+  forall Γ l e1 e2 l' e1' e2', l = l' ->
+    EXP Γ ⊢ e1  ->
+    EXP Γ ⊢ e1' ->
+    EXP (l  + Γ) ⊢ e2  ->
+    EXP (l' + Γ) ⊢ e2' ->
+    R Γ       (ExpRes e1) (ExpRes e1') ->
+    R (l + Γ) (ExpRes e2) (ExpRes e2') ->
+    R Γ (ExpRes (Exp (ELet l e1 e2))) (ExpRes (Exp (ELet l' e1' e2'))).
+
+Definition CompatibleESeq (R : nat -> ProgResult -> ProgResult -> Prop) :=
+  forall Γ e1 e2 e1' e2',
+    EXP Γ ⊢ e1  ->
+    EXP Γ ⊢ e1' ->
+    EXP Γ ⊢ e2  ->
+    EXP Γ ⊢ e2' ->
+    R Γ (ExpRes e1) (ExpRes e1') ->
+    R Γ (ExpRes e2) (ExpRes e2') ->
+    R Γ (ExpRes (Exp (ESeq e1 e2))) (ExpRes (Exp (ESeq e1' e2'))).
+
+Definition CompatibleELetRec (R : nat -> ProgResult -> ProgResult -> Prop) :=
+  forall Γ e l e' l', length l = length l' ->
+    EXP (length l  + Γ) ⊢ e  ->
+    EXP (length l' + Γ) ⊢ e' ->
+    (forall i, i < length l  -> EXP ((length l)  + (nth i (map fst l)  0) + Γ) ⊢ (nth i (map snd l)  (Val VNil))) ->
+    (forall i, i < length l' -> EXP ((length l') + (nth i (map fst l') 0) + Γ) ⊢ (nth i (map snd l') (Val VNil))) ->
+    R Γ (ExpRes e) (ExpRes e') ->
+    (forall i, i < length l  ->
+    R ((length l)  + (nth i (map fst l)  0) + Γ)
+    (ExpRes (nth i (map snd l) (Val VNil))) (ExpRes (nth i (map snd l') (Val VNil)))) ->
+    R Γ (ExpRes (Exp (ELetRec l e))) (ExpRes (Exp (ELetRec l' e'))).
+
+Definition CompatibleETry (R : nat -> ProgResult -> ProgResult -> Prop) :=
+  forall Γ e1 vl1 e2 vl2 e3 e1' vl1' e2' vl2' e3', 
+    vl1 = vl1' -> vl2 = vl2' ->
+    EXP Γ ⊢ e1  ->
+    EXP Γ ⊢ e1' ->
+    EXP (vl1  + Γ) ⊢ e2  ->
+    EXP (vl1' + Γ) ⊢ e2' ->
+    EXP (vl2  + Γ) ⊢ e3  ->
+    EXP (vl2' + Γ) ⊢ e3' ->
+    R Γ (ExpRes e1) (ExpRes e1') ->
+    R Γ (ExpRes e2) (ExpRes e2') ->
+    R Γ (ExpRes e3) (ExpRes e3') ->
+    R Γ (ExpRes (Exp (ETry e1 vl1 e2 vl2 e3))) (ExpRes (Exp (ETry e1' vl1' e2' vl2' e3'))).
+
+(*------------------------------ Value Expr Comp --------------------------------------------------------*)
+
+Definition CompatibleVNil (R : nat -> ProgResult -> ProgResult -> Prop) :=
+  forall Γ,
+    R Γ (ExpRes (Val VNil)) (ExpRes (Val VNil)).
+
+Definition CompatibleVLit (R : nat -> ProgResult -> ProgResult -> Prop) :=
+  forall Γ l l',
+    l = l' -> (* TODO: Is this ok for literals? *)
+    R Γ (ExpRes (Val (VLit l))) (ExpRes (Val (VLit l'))).
+
+Definition CompatibleVCons (R : nat -> ProgResult -> ProgResult -> Prop) :=
+  forall Γ e1 e1' e2 e2',
+    VAL Γ ⊢ e1 -> VAL Γ ⊢ e1' -> 
+    VAL Γ ⊢ e2 -> VAL Γ ⊢ e2' ->
+    R Γ (ExpRes (Val e1)) (ExpRes (Val e1')) -> 
+    R Γ (ExpRes (Val e2)) (ExpRes (Val e2')) ->
+    R Γ (ExpRes (Val (VCons e1 e2))) (ExpRes (Val (VCons e1' e2'))).
+
+Definition CompatibleVTuple (R : nat -> ProgResult -> ProgResult -> Prop) :=
+  forall Γ el el', length el = length el' ->
+    (forall i, i < length el  -> VAL Γ ⊢ (nth i el VNil)) ->
+    (forall i, i < length el' -> VAL Γ ⊢ (nth i el' VNil)) ->
+    (forall i, i < length el -> 
+    R Γ (ExpRes (Val (nth i el VNil))) (ExpRes (Val (nth i el' VNil)))) ->
+    R Γ (ExpRes (Val (VTuple el))) (ExpRes (Val (VTuple el'))).
+
+Definition CompatibleVMap (R : nat -> ProgResult -> ProgResult -> Prop) :=
+  forall Γ l l', length l = length l' ->
+    (forall i, i < length l  -> VAL Γ ⊢ (nth i (map fst l)  VNil)) ->
+    (forall i, i < length l' -> VAL Γ ⊢ (nth i (map fst l') VNil)) ->
+    (forall i, i < length l  -> VAL Γ ⊢ (nth i (map snd l)  VNil)) ->
+    (forall i, i < length l' -> VAL Γ ⊢ (nth i (map snd l') VNil)) ->
+    (forall i, i < length l -> 
+    R Γ (ExpRes (Val (nth i (map fst l) VNil))) (ExpRes (Val (nth i (map fst l') VNil)))) ->
+    (forall i, i < length l -> 
+    R Γ (ExpRes (Val (nth i (map snd l) VNil))) (ExpRes (Val (nth i (map snd l') VNil)))) ->
+    R Γ (ExpRes (Val (VMap l))) (ExpRes (Val (VMap l'))).
+
+Definition CompatibleVVar (R : nat -> ProgResult -> ProgResult -> Prop) :=
+  forall Γ n n',
+    n = n' ->
+    n  > Γ ->
+    n' > Γ ->
+    R Γ (ExpRes (Val (VVar n))) (ExpRes (Val (VVar n'))).
+
+Definition CompatibleVFunId (R : nat -> ProgResult -> ProgResult -> Prop) :=
+  forall Γ n n',
+    n = n' ->
+    n  > Γ ->
+    n' > Γ ->
+    R Γ (ExpRes (Val (VFunId n))) (ExpRes (Val (VFunId n'))).
+
+Definition CompatibleVClos (R : nat -> ProgResult -> ProgResult -> Prop) :=
+  forall Γ ext id vc e ext' id' vc' e',
+    length ext = length ext' ->
+    id = id' -> vc = vc' ->
+    EXP (length ext  + vc  + Γ) ⊢ e  -> 
+    EXP (length ext' + vc' + Γ) ⊢ e' -> 
+    (forall i, i < length ext  -> 
+    EXP (length ext  + (nth i (map snd (map fst ext))  0) + Γ) ⊢ (nth i (map snd ext)  (Val VNil))) ->
+    (forall i, i < length ext' -> 
+    EXP (length ext' + (nth i (map snd (map fst ext')) 0) + Γ) ⊢ (nth i (map snd ext') (Val VNil))) ->
+    R (length ext  + vc  + Γ) (ExpRes e) (ExpRes e') ->
+    (forall i, i < length ext ->
+    R (length ext  + (nth i (map snd (map fst ext))  0) + Γ)
+    (ExpRes (nth i (map snd ext)  (Val VNil))) (ExpRes (nth i (map snd ext') (Val VNil)))) ->
+    R Γ (ExpRes (Val (VClos ext id vc e))) (ExpRes (Val (VClos ext' id' vc' e'))).
+
+(*---------------------------- Meta Defs ------------------------------------------------------*)
+
+Definition IsPreCtxRel (R : nat -> ProgResult -> ProgResult -> Prop) :=
+  (forall Γ p1 p2, R Γ p1 p2 -> PROG Γ ⊢ p1 /\ PROG Γ ⊢ p2) /\
+  Adequate R /\ IsReflexive R /\
+  (forall Γ, Transitive (R Γ)) /\
+  CompatibleEFun R /\
+  CompatibleEValues R /\
+  CompatibleECons R /\
+  CompatibleETuple R /\
+  CompatibleEMap R /\
+  CompatibleECall R /\
+  CompatibleEPrimOp R /\
+  CompatibleEApp R /\
+  CompatibleECase R /\
+  CompatibleELet R /\
+  CompatibleESeq R /\
+  CompatibleELetRec R /\
+  CompatibleETry R /\
+  CompatibleVNil R /\
+  CompatibleVLit R /\
+  CompatibleVCons R /\
+  CompatibleVTuple R /\
+  CompatibleVMap R /\
+  CompatibleVVar R /\
+  CompatibleVFunId R /\
+  CompatibleVClos R.
+
+Definition IsCtxRel (R : nat -> ProgResult -> ProgResult -> Prop) :=
+  IsPreCtxRel R /\
+  forall R', IsPreCtxRel R' ->
+    forall Γ p1 p2, R' Γ p1 p2 -> R Γ p1 p2.
+
+
+
+
+
+
+
+
+Lemma bigger_implies_IsCtxRel : forall E R,
+    IsCtxRel R ->
+    IsPreCtxRel E ->
+    (forall Γ e1 e2, R Γ e1 e2 -> E Γ e1 e2) ->
+    IsCtxRel E.
+Proof.
+  intros.
+  split; auto.
+  intros.
+  apply H1.
+  destruct H.
+  eapply H4.
+  - exact H2.
+  - auto.
+Qed.
+
+(* Theorem Erel_IsPreCtxRel : IsPreCtxRel Erel_open. *)
+
+(* Corollary CIU_IsPreCtxRel : IsPreCtxRel CIU_open. *)
+
+
+Inductive Ctx :=
+| CHole
+| CFun    (vl : nat) (c : Ctx)
+| CValues (el : list Expression) (c : Ctx) (el' : list Expression)
+| CCons1  (c : Ctx) (tl : Expression)
+| CCons2  (hd : Expression) (c : Ctx)
+| CTuple  (l : list Expression) (c : Ctx) (l' : list Expression)
+| CMap1    (l : list (Expression * Expression)) (c : Ctx) (e2 : Expression) (l' : list (Expression * Expression))
+| CMap2    (l : list (Expression * Expression)) (e1 : Expression) (c : Ctx) (l' : list (Expression * Expression))
+| CCall   (f : string)    (l : list Expression) (c : Ctx) (l' : list Expression)
+| CPrimOp (f : string)    (l : list Expression) (c : Ctx) (l' : list Expression)
+| CApp1    (c : Ctx) (l : list Expression)
+| CApp2    (exp: Expression) (l : list Expression) (c : Ctx) (l' : list Expression)
+| CCase1   (c : Ctx) (l : list ((list Pattern) * Expression * Expression))
+| CCase2   (e : Expression) (l : list ((list Pattern) * Expression * Expression)) (lp : (list Pattern)) (c : Ctx) (e2 : Expression) (l' : list ((list Pattern) * Expression * Expression))
+| CCase3   (e : Expression) (l : list ((list Pattern) * Expression * Expression)) (lp : (list Pattern)) (e1 : Expression) (c : Ctx) (l' : list ((list Pattern) * Expression * Expression))
+| CLet1    (l : nat) (c : Ctx) (e2 : Expression)
+| CLet2    (l : nat) (e1: Expression) (c : Ctx)
+| CSeq1    (c : Ctx) (e2 : Expression)
+| CSeq2    (e1 : Expression) (c : Ctx)
+| CLetRec1 (l : list (nat * Expression)) (n : nat) (c : Ctx) (l' : list (nat * Expression)) (e : Expression)
+| CLetRec2 (l : list (nat * Expression)) (c : Ctx)
+| CTry1   (c : Ctx) (vl1 : nat) (e2 : Expression) (vl2 : nat) (e3 : Expression)
+| CTry2   (e1 : Expression) (vl1 : nat) (c : Ctx) (vl2 : nat) (e3 : Expression)
+| CTry3   (e1 : Expression) (vl1 : nat) (e2 : Expression) (vl2 : nat) (c : Ctx)
+.
+
+Fixpoint plug (C : Ctx) (p : Expression) :=
+match C with
+| CHole             => p
+| CFun    vl c      => Exp ( EFun vl (plug c p) )
+| CValues el c el'  => Exp ( EValues (el ++ [(plug c p)] ++ el') )
+| CCons1  c tl      => Exp ( ECons (plug c p) tl )
+| CCons2  hd c      => Exp ( ECons hd (plug c p) )
+| CTuple  l c l'    => Exp ( ETuple (l ++ [(plug c p)] ++ l') )
+| CMap1   l c e2 l' => Exp ( EMap (l ++ [((plug c p), e2)] ++ l') )
+| CMap2   l e1 c l' => Exp ( EMap (l ++ [(e1, (plug c p))] ++ l') )
+| CCall   f l c l'  => Exp ( ECall f (l ++ [(plug c p)] ++ l') )
+| CPrimOp f l c l'  => Exp ( EPrimOp f (l ++ [(plug c p)] ++ l') )
+| CApp1   c l       => Exp ( EApp (plug c p) l )
+| CApp2   exp l c l' => Exp ( EApp exp (l ++ [(plug c p)] ++ l') )
+| CCase1  c l       => Exp ( ECase (plug c p) l )
+| CCase2  e l lp c e2 l' => Exp ( ECase e (l ++ [(lp, (plug c p), e2)] ++ l') )
+| CCase3  e l lp e1 c l' => Exp ( ECase e (l ++ [(lp, e1, (plug c p))] ++ l') )
+| CLet1   l c e2    => Exp ( ELet l (plug c p) e2 )
+| CLet2   l e1 c    => Exp ( ELet l e1 (plug c p) )
+| CSeq1   c e2      => Exp ( ESeq (plug c p) e2 )
+| CSeq2   e1 c      => Exp ( ESeq e1 (plug c p) )
+| CLetRec1 l n c l' e => Exp ( ELetRec (l ++ [(n, (plug c p))] ++ l') e )
+| CLetRec2 l c     => Exp ( ELetRec l (plug c p) )
+| CTry1   c vl1 e2 vl2 e3  => Exp ( ETry (plug c p) vl1 e2 vl2 e3 )
+| CTry2   e1 vl1 c vl2 e3  => Exp ( ETry e1 vl1 (plug c p) vl2 e3 )
+| CTry3   e1 vl1 e2 vl2 c  => Exp ( ETry e1 vl1 e2 vl2 (plug c p) )
+end.
+
+Fixpoint plugc (C : Ctx) (p : Ctx) :=
+match C with
+| CHole             => p
+| CFun    vl c      => CFun vl (plugc c p)
+| CValues el c el'  => CValues el (plugc c p) el'
+| CCons1  c tl      => CCons1 (plugc c p) tl
+| CCons2  hd c      => CCons2 hd (plugc c p)
+| CTuple  l c l'    => CTuple l (plugc c p) l'
+| CMap1   l c e2 l' => CMap1 l (plugc c p) e2 l'
+| CMap2   l e1 c l' => CMap2 l e1 (plugc c p) l'
+| CCall   f l c l'  => CCall f l (plugc c p) l'
+| CPrimOp f l c l'  => CPrimOp f l (plugc c p) l'
+| CApp1   c l       => CApp1 (plugc c p) l
+| CApp2   exp l c l' => CApp2 exp l (plugc c p) l'
+| CCase1  c l       => CCase1 (plugc c p) l
+| CCase2  e l lp c e2 l' => CCase2 e l lp (plugc c p) e2 l'
+| CCase3  e l lp e1 c l' => CCase3 e l lp e1 (plugc c p) l'
+| CLet1   l c e2    => CLet1 l (plugc c p) e2
+| CLet2   l e1 c    => CLet2 l e1 (plugc c p)
+| CSeq1   c e2      => CSeq1 (plugc c p) e2
+| CSeq2   e1 c      => CSeq2 e1 (plugc c p)
+| CLetRec1 l n c l' e => CLetRec1 l n (plugc c p) l' e
+| CLetRec2 l c      => CLetRec2 l (plugc c p)
+| CTry1   c vl1 e2 vl2 e3  => CTry1 (plugc c p) vl1 e2 vl2 e3
+| CTry2   e1 vl1 c vl2 e3  => CTry2 e1 vl1 (plugc c p) vl2 e3
+| CTry3   e1 vl1 e2 vl2 c  => CTry3 e1 vl1 e2 vl2 (plugc c p)
+end.
+
+
+Lemma plug_assoc : forall C1 C2 e,
+    plug C1 (plug C2 e) =
+    plug (plugc C1 C2) e.
+Proof.
+  induction C1;
+    intros;
+    cbn;
+    auto;
+    rewrite IHC1;
+    auto.
+Qed.
+
+Reserved Notation "'EECTX' Γh ⊢ C ∷ Γ" (at level 60).
+(* Reserved Notation "'VECTX' Γh ⊢ C ∷ Γ" (at level 60). *)
+
+Inductive EECtxScope (Γh : nat) : nat -> Ctx -> Prop :=
+
+| CEScope_Hole : (EECTX Γh ⊢ CHole ∷ Γh)
+
+| CEScope_CFun : forall Γ vl c,
+  EECTX Γh ⊢ c ∷ (vl + Γ) -> 
+  EECTX Γh ⊢ (CFun vl c) ∷ Γ
+
+| CEScope_CValues : forall Γ el c el',
+  (forall i, i < length el  -> EXP Γ ⊢ (nth i el  (Val VNil))) ->
+  EECTX Γh ⊢ c ∷ Γ ->
+  (forall i, i < length el' -> EXP Γ ⊢ (nth i el' (Val VNil))) ->
+  EECTX Γh ⊢ (CValues el c el') ∷ Γ
+
+| CEScope_CCons1 : forall Γ c tl,
+  EECTX Γh ⊢ c ∷ Γ ->
+  EXP Γ ⊢ tl ->
+  EECTX Γh ⊢ (CCons1 c tl) ∷ Γ
+
+| CEScope_CCons2 : forall Γ hd c,
+  EXP Γ ⊢ hd ->
+  EECTX Γh ⊢ c ∷ Γ ->
+  EECTX Γh ⊢ (CCons2 hd c) ∷ Γ
+
+| CEScope_CTuple : forall Γ l c l',
+  (forall i, i < length l  -> EXP Γ ⊢ (nth i l  (Val VNil))) ->
+  EECTX Γh ⊢ c ∷ Γ ->
+  (forall i, i < length l' -> EXP Γ ⊢ (nth i l' (Val VNil))) ->
+  EECTX Γh ⊢ (CTuple l c l') ∷ Γ
+
+| CEScope_CMap1 : forall Γ l c e2 l',
+  (forall i, i < length l  -> EXP Γ ⊢ (nth i (map fst l)  (Val VNil))) ->
+  (forall i, i < length l  -> EXP Γ ⊢ (nth i (map snd l)  (Val VNil))) ->
+  EECTX Γh ⊢ c ∷ Γ ->
+  EXP Γ ⊢ e2 ->
+  (forall i, i < length l' -> EXP Γ ⊢ (nth i (map fst l') (Val VNil))) ->
+  (forall i, i < length l' -> EXP Γ ⊢ (nth i (map snd l') (Val VNil))) ->
+  EECTX Γh ⊢ (CMap1 l c e2 l') ∷ Γ
+
+| CEScope_CMap2 : forall Γ l e1 c l',
+  (forall i, i < length l  -> EXP Γ ⊢ (nth i (map fst l)  (Val VNil))) ->
+  (forall i, i < length l  -> EXP Γ ⊢ (nth i (map snd l)  (Val VNil))) ->
+  EXP Γ ⊢ e1 ->
+  EECTX Γh ⊢ c ∷ Γ ->
+  (forall i, i < length l' -> EXP Γ ⊢ (nth i (map fst l') (Val VNil))) ->
+  (forall i, i < length l' -> EXP Γ ⊢ (nth i (map snd l') (Val VNil))) ->
+  EECTX Γh ⊢ (CMap2 l e1 c l') ∷ Γ
+
+| CEScope_CCall : forall Γ f l c l',
+  (forall i, i < length l  -> EXP Γ ⊢ (nth i l  (Val VNil))) ->
+  EECTX Γh ⊢ c ∷ Γ ->
+  (forall i, i < length l' -> EXP Γ ⊢ (nth i l' (Val VNil))) ->
+  EECTX Γh ⊢ (CCall f l c l') ∷ Γ
+
+| CEScope_CPrimOp : forall Γ f l c l',
+  (forall i, i < length l  -> EXP Γ ⊢ (nth i l  (Val VNil))) ->
+  EECTX Γh ⊢ c ∷ Γ ->
+  (forall i, i < length l' -> EXP Γ ⊢ (nth i l' (Val VNil))) ->
+  EECTX Γh ⊢ (CPrimOp f l c l') ∷ Γ
+
+| CEScope_CApp1 : forall Γ c l,
+  EECTX Γh ⊢ c ∷ Γ ->
+  (forall i, i < length l  -> EXP Γ ⊢ (nth i l  (Val VNil))) ->
+  EECTX Γh ⊢ (CApp1 c l) ∷ Γ
+
+| CEScope_CApp2 : forall Γ exp l c l',
+  EXP Γ ⊢ exp ->
+  (forall i, i < length l  -> EXP Γ ⊢ (nth i l  (Val VNil))) ->
+  EECTX Γh ⊢ c ∷ Γ ->
+  (forall i, i < length l' -> EXP Γ ⊢ (nth i l' (Val VNil))) ->
+  EECTX Γh ⊢ (CApp2 exp l c l') ∷ Γ
+
+| CEScope_CCase1 : forall Γ c l,
+  EECTX Γh ⊢ c ∷ Γ ->
+  (forall i, i < length l -> 
+  EXP ((patternListScope (nth i (map fst (map fst l)) nil)) + Γ) ⊢ (nth i (map snd (map fst l)) (Val VNil))) ->
+  (forall i, i < length l -> 
+  EXP ((patternListScope (nth i (map fst (map fst l)) nil)) + Γ) ⊢ (nth i (map snd l) (Val VNil))) ->
+  EECTX Γh ⊢ (CCase1 c l) ∷ Γ
+
+
+| CEScope_CCase2 : forall Γ e l lp c e2 l',
+  EXP Γ ⊢ e ->
+  (forall i, i < length l -> 
+  EXP ((patternListScope (nth i (map fst (map fst l)) nil)) + Γ) ⊢ (nth i (map snd (map fst l)) (Val VNil))) ->
+  (forall i, i < length l -> 
+  EXP ((patternListScope (nth i (map fst (map fst l)) nil)) + Γ) ⊢ (nth i (map snd l) (Val VNil))) ->
+  EECTX Γh ⊢ c ∷ ((patternListScope lp) + Γ) ->
+  EXP ((patternListScope lp) + Γ) ⊢ e2 ->
+  (forall i, i < length l' -> 
+  EXP ((patternListScope (nth i (map fst (map fst l')) nil)) + Γ) ⊢ (nth i (map snd (map fst l')) (Val VNil))) ->
+  (forall i, i < length l' -> 
+  EXP ((patternListScope (nth i (map fst (map fst l')) nil)) + Γ) ⊢ (nth i (map snd l') (Val VNil))) ->
+  EECTX Γh ⊢ (CCase2 e l lp c e2 l') ∷ Γ
+
+| CEScope_CCase3 : forall Γ e l lp e1 c l',
+  EXP Γ ⊢ e ->
+  (forall i, i < length l -> 
+  EXP ((patternListScope (nth i (map fst (map fst l)) nil)) + Γ) ⊢ (nth i (map snd (map fst l)) (Val VNil))) ->
+  (forall i, i < length l -> 
+  EXP ((patternListScope (nth i (map fst (map fst l)) nil)) + Γ) ⊢ (nth i (map snd l) (Val VNil))) ->
+  EXP ((patternListScope lp) + Γ) ⊢ e1 ->
+  EECTX Γh ⊢ c ∷ ((patternListScope lp) + Γ) ->
+  (forall i, i < length l' -> 
+  EXP ((patternListScope (nth i (map fst (map fst l')) nil)) + Γ) ⊢ (nth i (map snd (map fst l')) (Val VNil))) ->
+  (forall i, i < length l' -> 
+  EXP ((patternListScope (nth i (map fst (map fst l')) nil)) + Γ) ⊢ (nth i (map snd l') (Val VNil))) ->
+  EECTX Γh ⊢ (CCase3 e l lp e1 c l') ∷ Γ
+
+| CEScope_CLet1 : forall Γ l c e2,
+  EECTX Γh ⊢ c ∷ Γ ->
+  EXP (l + Γ) ⊢ e2 ->
+  EECTX Γh ⊢ (CLet1 l c e2) ∷ Γ
+
+| CEScope_CLet2 : forall Γ l e1 c,
+  EXP Γ ⊢ e1 ->
+  EECTX Γh ⊢ c ∷ (l + Γ) ->
+  EECTX Γh ⊢ (CLet2 l e1 c) ∷ Γ
+
+| CEScope_CSeq1 : forall Γ c e2,
+  EECTX Γh ⊢ c ∷ Γ ->
+  EXP Γ ⊢ e2 ->
+  EECTX Γh ⊢ (CSeq1 c e2) ∷ Γ
+
+| CEScope_CSeq2 : forall Γ e1 c,
+  EXP Γ ⊢ e1 ->
+  EECTX Γh ⊢ c ∷ Γ ->
+  EECTX Γh ⊢ (CSeq2 e1 c) ∷ Γ
+
+| CEScope_CLetRec1 : forall Γ l n c l' e,
+  (forall i, i < length l  -> 
+  EXP (1 + (length l) + (length l') + (nth i (map fst l)  0) + Γ) ⊢ (nth i (map snd l)  (Val VNil))) ->
+  EECTX Γh ⊢ c ∷ (1 + (length l) + (length l') + n + Γ) ->
+  (forall i, i < length l' -> 
+  EXP (1 + (length l) + (length l') + (nth i (map fst l') 0) + Γ) ⊢ (nth i (map snd l') (Val VNil))) ->
+  EXP (1 + length l + length l' + Γ) ⊢ e ->
+  EECTX Γh ⊢ (CLetRec1 l n c l' e) ∷ Γ
+
+| CEScope_CLetRec2 : forall Γ l c,
+  (forall i, i < length l  -> EXP ((length l)+ (nth i (map fst l)  0) + Γ) ⊢ (nth i (map snd l)  (Val VNil))) ->
+  EECTX Γh ⊢ c ∷ (length l + Γ) ->
+  EECTX Γh ⊢ (CLetRec2 l c) ∷ Γ
+
+| CEScope_CTry1 : forall Γ c vl1 e2 vl2 e3,
+  EECTX Γh ⊢ c ∷ Γ ->
+  EXP (vl1 + Γ) ⊢ e2 ->
+  EXP (vl2 + Γ) ⊢ e3 ->
+  EECTX Γh ⊢ (CTry1 c vl1 e2 vl2 e3) ∷ Γ
+
+| CEScope_CTry2 : forall Γ e1 vl1 c vl2 e3,
+  EXP Γ ⊢ e1 ->
+  EECTX Γh ⊢ c ∷ (vl1 + Γ) ->
+  EXP (vl2 + Γ) ⊢ e3 ->
+  EECTX Γh ⊢ (CTry2 e1 vl1 c vl2 e3) ∷ Γ
+
+| CEScope_CTry3 : forall Γ e1 vl1 e2 vl2 c,
+  EXP Γ ⊢ e1 ->
+  EXP (vl1 + Γ) ⊢ e2 ->
+  EECTX Γh ⊢ c ∷ (vl2 + Γ) ->
+  EECTX Γh ⊢ (CTry3 e1 vl1 e2 vl2 c) ∷ Γ
+
+where
+"'EECTX' Γh ⊢ C ∷ Γ" := (EECtxScope Γh Γ C)
+.
+
+
+Ltac solve_inversion :=
+  match goal with
+  | [ H : _ |- _ ] => solve [inversion H]
+  end.
+
+
+Lemma plug_preserves_scope_exp : forall {Γh C Γ e},
+    (EECTX Γh ⊢ C ∷ Γ ->
+     EXP Γh ⊢ e ->
+     EXP Γ ⊢ plug C e).
+Proof.
+  induction C; intros; inversion H; subst.
+  * simpl. auto.
+  * specialize (IHC (vl + Γ) e H3 H0).
+    simpl. constructor. constructor. auto.
+  * specialize (IHC Γ e H6 H0).
+    simpl. constructor. constructor.
+    Check indexed_to_forall.
+    rewrite <- (indexed_to_forall _ (fun e => EXP Γ ⊢ e) _).
+    apply Forall_app. split.
+    - rewrite (indexed_to_forall _ _ (Val VNil)). auto.
+    - replace (plug C e :: el') with ([plug C e] ++ el') by (simpl; auto).
+      apply Forall_app. split.
+      + auto.
+      + rewrite (indexed_to_forall _ _ (Val VNil)). auto.
+  * simpl. constructor. constructor; auto.
+  * simpl. constructor. constructor; auto.
+  * simpl. constructor. constructor.
+    rewrite <- (indexed_to_forall _ (fun e => EXP Γ ⊢ e) _). apply Forall_app. split.
+    - rewrite (indexed_to_forall _ _ (Val VNil)). auto.
+    - replace (plug C e :: l') with ([plug C e] ++ l') by (simpl; auto).
+      apply Forall_app. split.
+      + auto.
+      + rewrite (indexed_to_forall _ _ (Val VNil)). auto.
+  * simpl. constructor. constructor.
+    - Check indexed_to_forall. Check map_nth.
+      (* this section brings the fst to the front of the nth exp *)
+      intros.
+      replace (Val VNil) with (fst (Val VNil, Val VNil)) by (simpl;auto).
+      rewrite map_nth. generalize H1. generalize i. clear i H1.
+      
+      rewrite <- (indexed_to_forall _ (fun e => EXP Γ ⊢ fst e) (Val VNil, Val VNil)).
+      apply Forall_app. split.
+      + rewrite (indexed_to_forall _ _ (Val VNil, Val VNil)). intros.
+        specialize (H5 i H1). rewrite <- map_nth. simpl. auto.
+      + replace ((plug C e, e2):: l') with ([(plug C e, e2)] ++ l') by (simpl; auto).
+        apply Forall_app. split.
+        ** rewrite (indexed_to_forall _ _ (Val VNil, Val VNil)). intros. inversion H1.
+           -- subst. simpl. auto.
+           -- lia.
+        ** rewrite (indexed_to_forall _ _ (Val VNil, Val VNil)). intros.
+           specialize (H10 i H1). rewrite <- map_nth. simpl. auto.
+  - (* this section brings the fst to the front of the nth exp *)
+    intros.
+    replace (Val VNil) with (snd (Val VNil, Val VNil)) by (simpl;auto).
+    rewrite map_nth. generalize H1. generalize i. clear i H1.
+    
+    rewrite <- (indexed_to_forall _ (fun e => EXP Γ ⊢ snd e) (Val VNil, Val VNil)).
+    apply Forall_app. split.
+    + rewrite (indexed_to_forall _ _ (Val VNil, Val VNil)). intros.
+        specialize (H6 i H1). rewrite <- map_nth. simpl. auto.
+      + replace ((plug C e, e2):: l') with ([(plug C e, e2)] ++ l') by (simpl; auto).
+        apply Forall_app. split.
+        ** rewrite (indexed_to_forall _ _ (Val VNil, Val VNil)). intros. inversion H1.
+           -- subst. simpl. auto.
+           -- lia.
+        ** rewrite (indexed_to_forall _ _ (Val VNil, Val VNil)). intros.
+           specialize (H11 i H1). rewrite <- map_nth. simpl. auto.
+  * simpl. constructor. constructor.
+    -(* this section brings the fst to the front of the nth exp *)
+      intros.
+      replace (Val VNil) with (fst (Val VNil, Val VNil)) by (simpl;auto).
+      rewrite map_nth. generalize H1. generalize i. clear i H1.
+      
+      rewrite <- (indexed_to_forall _ (fun e => EXP Γ ⊢ fst e) (Val VNil, Val VNil)).
+      apply Forall_app. split.
+      + rewrite (indexed_to_forall _ _ (Val VNil, Val VNil)). intros.
+        specialize (H5 i H1). rewrite <- map_nth. simpl. auto.
+      + replace ((e1, plug C e):: l') with ([(e1, plug C e)] ++ l') by (simpl; auto).
+        apply Forall_app. split.
+        ** rewrite (indexed_to_forall _ _ (Val VNil, Val VNil)). intros. inversion H1.
+           -- subst. simpl. auto.
+           -- lia.
+        ** rewrite (indexed_to_forall _ _ (Val VNil, Val VNil)). intros.
+           specialize (H10 i H1). rewrite <- map_nth. simpl. auto.
+  - (* this section brings the fst to the front of the nth exp *)
+    intros.
+    replace (Val VNil) with (snd (Val VNil, Val VNil)) by (simpl;auto).
+    rewrite map_nth. generalize H1. generalize i. clear i H1.
+    
+    rewrite <- (indexed_to_forall _ (fun e => EXP Γ ⊢ snd e) (Val VNil, Val VNil)).
+    apply Forall_app. split.
+    + rewrite (indexed_to_forall _ _ (Val VNil, Val VNil)). intros.
+        specialize (H6 i H1). rewrite <- map_nth. simpl. auto.
+      + replace ((e1, plug C e):: l') with ([(e1, plug C e)] ++ l') by (simpl; auto).
+        apply Forall_app. split.
+        ** rewrite (indexed_to_forall _ _ (Val VNil, Val VNil)). intros. inversion H1.
+           -- subst. simpl. auto.
+           -- lia.
+        ** rewrite (indexed_to_forall _ _ (Val VNil, Val VNil)). intros.
+           specialize (H11 i H1). rewrite <- map_nth. simpl. auto.
+  * simpl. constructor. constructor.
+     rewrite <- (indexed_to_forall _ (fun e => EXP Γ ⊢ e) _). apply Forall_app. split.
+    - rewrite (indexed_to_forall _ _ (Val VNil)). auto.
+    - replace (plug C e :: l') with ([plug C e] ++ l') by (simpl; auto).
+      apply Forall_app. split.
+      + auto.
+      + rewrite (indexed_to_forall _ _ (Val VNil)). auto.
+  * simpl. constructor. constructor.
+    rewrite <- (indexed_to_forall _ (fun e => EXP Γ ⊢ e) _). apply Forall_app. split.
+    - rewrite (indexed_to_forall _ _ (Val VNil)). auto.
+    - replace (plug C e :: l') with ([plug C e] ++ l') by (simpl; auto).
+      apply Forall_app. split.
+      + auto.
+      + rewrite (indexed_to_forall _ _ (Val VNil)). auto.
+  * simpl. constructor. constructor.
+    - auto.
+    - auto.
+  * simpl. constructor. constructor.
+    - auto.
+    - rewrite <- (indexed_to_forall _ (fun e => EXP Γ ⊢ e) _). apply Forall_app. split.
+      + rewrite (indexed_to_forall _ _ (Val VNil)). auto.
+      + replace (plug C e :: l') with ([plug C e] ++ l') by (simpl; auto).
+        apply Forall_app. split.
+        ** auto.
+        ** rewrite (indexed_to_forall _ _ (Val VNil)). auto.
+  * simpl. constructor. constructor.
+    - auto.
+    - auto. 
+    - auto. 
+  * simpl. constructor. constructor.
+    - auto.
+    - (* this section brings the snd fst to the front of the nth exp *)
+      intros. rewrite map_map.
+      remember (fun x : list Pattern * Expression * Expression => snd (fst x)) as F.
+      replace (Val VNil) with (F ([], Val VNil, Val VNil)) by (subst;simpl;auto).
+      rewrite map_nth. subst.
+      (* this section brings the fst fst to the front of the nth exp *)
+      rewrite map_map. remember (fun x : list Pattern * Expression * Expression =>
+      fst (fst x)) as F. remember (nth i (map F (l ++ (lp, plug C e0, e2) :: l')) []) as T.
+      replace [] with (F ([], Val VNil, Val VNil)) in HeqT by (subst;simpl;auto).
+      rewrite map_nth in HeqT. subst.
+      generalize H1. generalize i. clear i H1. 
+      
+      rewrite <- (indexed_to_forall _ (fun e => 
+      EXP (patternListScope (fst (fst e)) + Γ) ⊢ snd (fst e)) _).
+      apply Forall_app. split.
+      + (* Here I just need to bring H9 to the same format*)
+        rewrite (indexed_to_forall _ _ ([], Val VNil, Val VNil)).
+        intros. specialize (H9 i H1).
+        do 2 rewrite map_map in H9.
+        remember (fun x : list Pattern * Expression * Expression => snd (fst x)) as F.
+        replace (Val VNil) with (F ([], Val VNil, Val VNil)) in H9 by (subst;simpl;auto).
+        rewrite map_nth in H9. subst.
+        remember (fun x : list Pattern * Expression * Expression =>
+        fst (fst x)) as F. remember (nth i (map F l) []) as T.
+        replace [] with (F ([], Val VNil, Val VNil)) in HeqT by (subst;simpl;auto).
+        rewrite map_nth in HeqT. subst. auto.
+      + replace ((lp, plug C e0, e2) :: l') with ([(lp, plug C e0, e2)] ++ l') 
+        by (simpl; auto). apply Forall_app. split.
+        ** rewrite (indexed_to_forall _ _ ([], Val VNil, Val VNil)). intros.
+           inversion H1.
+           -- subst. simpl. auto.
+           -- lia.
+        ** (* Here I just need to bring H13 to the same format*)
+           rewrite (indexed_to_forall _ _ ([], Val VNil, Val VNil)).
+           intros. specialize (H13 i H1).
+           do 2 rewrite map_map in H13.
+           remember (fun x : list Pattern * Expression * Expression => snd (fst x)) as F.
+           replace (Val VNil) with (F ([], Val VNil, Val VNil)) in H13 by (subst;simpl;auto).
+           rewrite map_nth in H13. subst.
+           remember (fun x : list Pattern * Expression * Expression =>
+           fst (fst x)) as F. remember (nth i (map F l') []) as T.
+           replace [] with (F ([], Val VNil, Val VNil)) in HeqT by (subst;simpl;auto).
+           rewrite map_nth in HeqT. subst. auto.
+    - (* this section brings the snd fst to the front of the nth exp *)
+      intros. rewrite map_map.
+      remember (fun x : list Pattern * Expression * Expression => snd (x)) as F.
+      replace (Val VNil) with (F ([], Val VNil, Val VNil)) by (subst;simpl;auto).
+      rewrite map_nth. subst.
+      (* this section brings the fst fst to the front of the nth exp *)
+      remember (fun x : list Pattern * Expression * Expression =>
+      fst (fst x)) as F. remember (nth i (map F (l ++ (lp, plug C e0, e2) :: l')) []) as T.
+      replace [] with (F ([], Val VNil, Val VNil)) in HeqT by (subst;simpl;auto).
+      rewrite map_nth in HeqT. subst.
+      generalize H1. generalize i. clear i H1. 
+      
+      rewrite <- (indexed_to_forall _ (fun e => 
+      EXP (patternListScope (fst (fst e)) + Γ) ⊢ snd (e)) _).
+      apply Forall_app. split.
+      + (* Here I just need to bring H10 to the same format*)
+        rewrite (indexed_to_forall _ _ ([], Val VNil, Val VNil)).
+        intros. specialize (H10 i H1).
+        rewrite map_map in H10.
+        remember (fun x : list Pattern * Expression * Expression => snd (x)) as F.
+        replace (Val VNil) with (F ([], Val VNil, Val VNil)) in H10 by (subst;simpl;auto).
+        rewrite map_nth in H10. subst.
+        remember (fun x : list Pattern * Expression * Expression =>
+        fst (fst x)) as F. remember (nth i (map F l) []) as T.
+        replace [] with (F ([], Val VNil, Val VNil)) in HeqT by (subst;simpl;auto).
+        rewrite map_nth in HeqT. subst. auto.
+      + replace ((lp, plug C e0, e2) :: l') with ([(lp, plug C e0, e2)] ++ l') 
+        by (simpl; auto). apply Forall_app. split.
+        ** rewrite (indexed_to_forall _ _ ([], Val VNil, Val VNil)). intros.
+           inversion H1.
+           -- subst. simpl. auto.
+           -- lia.
+        ** (* Here I just need to bring H14 to the same format*)
+           rewrite (indexed_to_forall _ _ ([], Val VNil, Val VNil)).
+           intros. specialize (H14 i H1).
+           rewrite map_map in H14.
+           remember (fun x : list Pattern * Expression * Expression => snd (x)) as F.
+           replace (Val VNil) with (F ([], Val VNil, Val VNil)) in H14 by (subst;simpl;auto).
+           rewrite map_nth in H14. subst.
+           remember (fun x : list Pattern * Expression * Expression =>
+           fst (fst x)) as F. remember (nth i (map F l') []) as T.
+           replace [] with (F ([], Val VNil, Val VNil)) in HeqT by (subst;simpl;auto).
+           rewrite map_nth in HeqT. subst. auto.
+  * simpl. constructor. constructor.
+    - auto.
+    - (* this section brings the snd fst to the front of the nth exp *)
+      intros. rewrite map_map.
+      remember (fun x : list Pattern * Expression * Expression => snd (fst x)) as F.
+      replace (Val VNil) with (F ([], Val VNil, Val VNil)) by (subst;simpl;auto).
+      rewrite map_nth. subst.
+      (* this section brings the fst fst to the front of the nth exp *)
+      rewrite map_map. remember (fun x : list Pattern * Expression * Expression =>
+      fst (fst x)) as F. remember (nth i (map F (l ++ (lp, e1, plug C e0) :: l')) []) as T.
+      replace [] with (F ([], Val VNil, Val VNil)) in HeqT by (subst;simpl;auto).
+      rewrite map_nth in HeqT. subst.
+      generalize H1. generalize i. clear i H1. 
+      
+      rewrite <- (indexed_to_forall _ (fun e => 
+      EXP (patternListScope (fst (fst e)) + Γ) ⊢ snd (fst e)) _).
+      apply Forall_app. split.
+      + (* Here I just need to bring H9 to the same format*)
+        rewrite (indexed_to_forall _ _ ([], Val VNil, Val VNil)).
+        intros. specialize (H9 i H1).
+        do 2 rewrite map_map in H9.
+        remember (fun x : list Pattern * Expression * Expression => snd (fst x)) as F.
+        replace (Val VNil) with (F ([], Val VNil, Val VNil)) in H9 by (subst;simpl;auto).
+        rewrite map_nth in H9. subst.
+        remember (fun x : list Pattern * Expression * Expression =>
+        fst (fst x)) as F. remember (nth i (map F l) []) as T.
+        replace [] with (F ([], Val VNil, Val VNil)) in HeqT by (subst;simpl;auto).
+        rewrite map_nth in HeqT. subst. auto.
+      + replace ((lp, e1, plug C e0) :: l') with ([(lp, e1, plug C e0)] ++ l') 
+        by (simpl; auto). apply Forall_app. split.
+        ** rewrite (indexed_to_forall _ _ ([], Val VNil, Val VNil)). intros.
+           inversion H1.
+           -- subst. simpl. auto.
+           -- lia.
+        ** (* Here I just need to bring H13 to the same format*)
+           rewrite (indexed_to_forall _ _ ([], Val VNil, Val VNil)).
+           intros. specialize (H13 i H1).
+           do 2 rewrite map_map in H13.
+           remember (fun x : list Pattern * Expression * Expression => snd (fst x)) as F.
+           replace (Val VNil) with (F ([], Val VNil, Val VNil)) in H13 by (subst;simpl;auto).
+           rewrite map_nth in H13. subst.
+           remember (fun x : list Pattern * Expression * Expression =>
+           fst (fst x)) as F. remember (nth i (map F l') []) as T.
+           replace [] with (F ([], Val VNil, Val VNil)) in HeqT by (subst;simpl;auto).
+           rewrite map_nth in HeqT. subst. auto.
+    - (* this section brings the snd fst to the front of the nth exp *)
+      intros. rewrite map_map.
+      remember (fun x : list Pattern * Expression * Expression => snd (x)) as F.
+      replace (Val VNil) with (F ([], Val VNil, Val VNil)) by (subst;simpl;auto).
+      rewrite map_nth. subst.
+      (* this section brings the fst fst to the front of the nth exp *)
+      remember (fun x : list Pattern * Expression * Expression =>
+      fst (fst x)) as F. remember (nth i (map F (l ++ (lp, e1, plug C e0) :: l')) []) as T.
+      replace [] with (F ([], Val VNil, Val VNil)) in HeqT by (subst;simpl;auto).
+      rewrite map_nth in HeqT. subst.
+      generalize H1. generalize i. clear i H1. 
+      
+      rewrite <- (indexed_to_forall _ (fun e => 
+      EXP (patternListScope (fst (fst e)) + Γ) ⊢ snd (e)) _).
+      apply Forall_app. split.
+      + (* Here I just need to bring H10 to the same format*)
+        rewrite (indexed_to_forall _ _ ([], Val VNil, Val VNil)).
+        intros. specialize (H10 i H1).
+        rewrite map_map in H10.
+        remember (fun x : list Pattern * Expression * Expression => snd (x)) as F.
+        replace (Val VNil) with (F ([], Val VNil, Val VNil)) in H10 by (subst;simpl;auto).
+        rewrite map_nth in H10. subst.
+        remember (fun x : list Pattern * Expression * Expression =>
+        fst (fst x)) as F. remember (nth i (map F l) []) as T.
+        replace [] with (F ([], Val VNil, Val VNil)) in HeqT by (subst;simpl;auto).
+        rewrite map_nth in HeqT. subst. auto.
+      + replace ((lp, e1, plug C e0) :: l') with ([(lp, e1, plug C e0)] ++ l') 
+        by (simpl; auto). apply Forall_app. split.
+        ** rewrite (indexed_to_forall _ _ ([], Val VNil, Val VNil)). intros.
+           inversion H1.
+           -- subst. simpl. auto.
+           -- lia.
+        ** (* Here I just need to bring H14 to the same format*)
+           rewrite (indexed_to_forall _ _ ([], Val VNil, Val VNil)).
+           intros. specialize (H14 i H1).
+           rewrite map_map in H14.
+           remember (fun x : list Pattern * Expression * Expression => snd (x)) as F.
+           replace (Val VNil) with (F ([], Val VNil, Val VNil)) in H14 by (subst;simpl;auto).
+           rewrite map_nth in H14. subst.
+           remember (fun x : list Pattern * Expression * Expression =>
+           fst (fst x)) as F. remember (nth i (map F l') []) as T.
+           replace [] with (F ([], Val VNil, Val VNil)) in HeqT by (subst;simpl;auto).
+           rewrite map_nth in HeqT. subst. auto.
+  * simpl. constructor. constructor; auto.
+  * simpl. constructor. constructor; auto.
+  * simpl. constructor. constructor; auto.
+  * simpl. constructor. constructor; auto.
+  * simpl. constructor. constructor.
+    - (* this section brings the fst to the front of the nth exp *)
+      intros. replace 0 with (fst (0, Val VNil)) by (simpl;auto).
+      rewrite map_nth.
+      (* this section brings the snd to the front of the nth exp *)
+      remember (nth i (map snd (l ++ (n, plug C e0) :: l')) (Val VNil)) as T.
+      replace (Val VNil) with (snd (0, Val VNil)) in HeqT by (simpl;auto).
+      rewrite map_nth in HeqT. subst.
+      generalize H1. generalize i. clear i H1.
+      rewrite <- (indexed_to_forall _ (fun e => 
+      EXP ( length (l ++ (n, plug C e0) :: l') + (fst e) + Γ) ⊢ snd  e) _).
+      apply Forall_app. split.
+      + (* Here I just need to bring H6 to the same format*)
+        rewrite (indexed_to_forall _ _ (0, Val VNil)). intros.
+        specialize (H6 i H1).
+        remember (nth i (map fst l) 0) as T.
+        replace 0 with (fst (0, Val VNil)) in HeqT by (simpl;auto).
+        rewrite map_nth in HeqT. subst.
+        remember (nth i (map snd l) (Val VNil)) as T in H6.
+        replace (Val VNil) with (snd (0, Val VNil)) in HeqT by (simpl;auto).
+        rewrite map_nth in HeqT. subst.
+        replace (Datatypes.length (l ++ (n, plug C e0) :: l')) with
+        (1 + Datatypes.length l + Datatypes.length l').
+        ** auto.
+        ** clear. rewrite app_length. replace ((n, plug C e0) :: l') with
+           ([(n, plug C e0)] ++ l') by (simpl;auto). rewrite app_length. simpl. auto.
+    + replace ((n, plug C e0) :: l') with ([(n, plug C e0)] ++ l') by (simpl;auto).
+      apply Forall_app. split.
+      ** rewrite (indexed_to_forall _ _ (0, Val VNil)). intros. inversion H1.
+         -- subst. simpl. replace (Datatypes.length (l ++ (n, plug C e0) :: l')) with
+            (1 + Datatypes.length l + Datatypes.length l').
+            ++ auto.
+            ++ clear. rewrite app_length. replace ((n, plug C e0) :: l') with
+              ([(n, plug C e0)] ++ l') by (simpl;auto). rewrite app_length. simpl. auto.
+         -- lia.
+      ** (* Here I just need to bring H9 to the same format*)
+          rewrite (indexed_to_forall _ _ (0, Val VNil)). intros.
+          specialize (H9 i H1).
+          remember (nth i (map fst l') 0) as T.
+          replace 0 with (fst (0, Val VNil)) in HeqT by (simpl;auto).
+          rewrite map_nth in HeqT. subst.
+          remember (nth i (map snd l') (Val VNil)) as T in H9.
+          replace (Val VNil) with (snd (0, Val VNil)) in HeqT by (simpl;auto).
+          rewrite map_nth in HeqT. subst.
+          replace (Datatypes.length (l ++ [(n, plug C e0)] ++ l')) with
+          (1 + Datatypes.length l + Datatypes.length l').
+          -- auto.
+          -- clear. rewrite app_length. replace ((n, plug C e0) :: l') with
+             ([(n, plug C e0)] ++ l') by (simpl;auto). rewrite app_length. simpl. auto.
+    - replace (Datatypes.length (l ++ (n, plug C e0) :: l')) with
+      (1 + Datatypes.length l + Datatypes.length l').
+      -- auto.
+      -- clear. rewrite app_length. replace ((n, plug C e0) :: l') with
+         ([(n, plug C e0)] ++ l') by (simpl;auto). rewrite app_length. simpl. auto.
+  * simpl. constructor. constructor; auto.
+  * simpl. constructor. constructor; auto.
+  * simpl. constructor. constructor; auto.
+  * simpl. constructor. constructor; auto.
+Qed.
+
+(* Lemma plugc_preserves_scope_exp *)
+
+(*V1*)
+Definition CTX (Γ : nat) (e1 e2 : Expression) :=
+  (EXP Γ ⊢ e1 /\ EXP Γ ⊢ e2) /\
+  (forall (C : Ctx),
+      EECTX Γ ⊢ C ∷ 0 -> | [], ExpRes (plug C e1) | ↓ -> | [], ExpRes (plug C e2) | ↓).
+
+(*V2*)
+(*
+Definition CTX (Γ : nat) (p1 p2 : ProgResult) :=
+  (PROG Γ ⊢ p1 /\ PROG Γ ⊢ p2) /\
+  (forall (C : Ctx),
+      EECTX Γ ⊢ C ∷ 0 -> | [], plug C p1 | ↓ -> | [], plug C p2| ↓).
+*)
+
+Lemma CTX_to_CIU : forall Γ e1 e2,
+  CTX Γ e1 e2 -> CIU e1 e2.
+Proof.
+  intros. inversion H. clear H. destruct H0. constructor.
+  * 
+  * split.
+    - admit.
+    - admit.
+Qed.
+
+
+
+
+
+
+
+
+
