src/updated/src/LogRel.v
@@ -1,0 +1,629 @@
+(*Require Export SubstSemantics.*)
+Require Export Termination.
+Require Export Equalities.
+
+Import ListNotations.
+
+(** Because of this, preorder is enough *)
+Goal forall T : Type, forall R : relation T, Reflexive R -> Transitive R ->
+  let R' := fun x y => R x y /\ R y x in Reflexive R' /\ Symmetric R' /\ Transitive R'.
+Proof.
+  intros. split. 2: split.
+  * intro. unfold R'. split; apply H.
+  * intro. intros. unfold R' in *. destruct H1.
+    split; auto.
+  * intro. intros. unfold R' in *. destruct H1, H2. split.
+    - eapply H0; eauto.
+    - eapply H0; eauto.
+Qed.
+
+
+Definition ProgRes_of (norm : (list ValueExpression + Exception)) : ProgResult := 
+match norm with
+| inr exc => ExcRes exc
+| inl vl => ValSeqRes vl
+end.
+
+(*
+Definition frame_rel (n : nat)
+                     (Nrel : forall m, m <= n -> (list ValueExpression + Exception) -> (list ValueExpression + Exception) -> Prop)
+                     (F1 F2 : FrameStack) : Prop :=
+  FSCLOSED F1 /\ FSCLOSED F2 /\
+  (forall m (Hmn : m <= n) (vl1 vl2 : (list ValueExpression + Exception)),
+    Nrel m Hmn vl1 vl2 ->
+    | F1, ProgRes_of vl1 | m ↓ -> | F2, ProgRes_of vl2 | ↓).
+*)
+
+Definition exc_rel (n : nat)
+                    (Vrel : forall m, m <= n -> ValueExpression -> ValueExpression -> Prop)
+                    (e1 e2 : Exception) : Prop :=
+match e1, e2 with
+  | (class1, reason1, details1), (class2, reason2, details2)  =>
+    class1 = class2 /\
+    (forall m (Hmn : m <= n),
+    Vrel m Hmn (reason1)  (reason2) /\
+    Vrel m Hmn (details1) (details2))
+end.
+
+Definition frame_rel (n : nat)
+                     (Vrel : forall m, m <= n -> ValueExpression -> ValueExpression -> Prop)
+                     (F1 F2 : FrameStack) : Prop :=
+  FSCLOSED F1 /\ FSCLOSED F2 /\
+  (forall m (Hmn : m <= n) (vl1 vl2 : list ValueExpression),
+    list_biforall (Vrel m Hmn) vl1 vl2 ->
+    | F1, ValSeqRes vl1 | m ↓ -> | F2, ValSeqRes vl2 | ↓)
+  /\
+  (forall m (Hmn : m <= n) (e1 e2 : Exception),
+    exc_rel m (fun m' H => Vrel m' (Nat.le_trans _ _ _ H Hmn)) e1 e2 ->
+    | F1, ExcRes e1 | m ↓ -> | F2, ExcRes e2 | ↓).
+
+(*
+Definition exp_rel (n : nat)
+                   (Nrel : forall m, m <= n -> (list ValueExpression + Exception) -> (list ValueExpression + Exception) -> Prop)
+                   (p1 p2 : Expression)
+                 : Prop :=
+  EXPCLOSED p1 /\ EXPCLOSED p2 /\
+  forall m (Hmn : m <= n) F1 F2,
+     frame_rel m (fun m' H => Nrel m' (Nat.le_trans _ _ _ H Hmn)) F1 F2 ->
+     | F1, ExpRes p1 | m ↓ -> | F2, ExpRes p2 | ↓
+.
+*)
+
+
+Definition exp_rel (n : nat)
+                   (Vrel : forall m, m <= n -> ValueExpression -> ValueExpression -> Prop)
+                   (p1 p2 : Expression)
+                 : Prop :=
+  EXPCLOSED p1 /\ EXPCLOSED p2 /\
+  forall m (Hmn : m <= n) F1 F2,
+     frame_rel m (fun m' H => Vrel m' (Nat.le_trans _ _ _ H Hmn)) F1 F2 ->
+     | F1, ExpRes p1 | m ↓ -> | F2, ExpRes p2 | ↓
+.
+
+(*
+Fixpoint Nrel_rec  (n : nat)
+                    (Nrel : forall m, m <= n -> (list ValueExpression + Exception) -> (list ValueExpression + Exception) -> Prop)
+                    (n1 n2 : (list ValueExpression + Exception)) : Prop :=
+  match n1, n2 with
+  | inl vl1,  inl vl2   => True
+  | inr (class1, reason1, details1), inr (class2, reason2, details2)  =>
+    class1 = class2 /\
+    Nrel_rec n Nrel (inl [reason1])  (inl [reason2]) /\
+    Nrel_rec n Nrel (inl [details1]) (inl [details2])
+  | _,  _ => False
+  end.
+  
+  
+  VALCLOSED v1 /\ VALCLOSED v2 /\
+  match v1, v2 with
+  | VNil, VNil => True
+  | VLit l, VLit l' => if Equalities.Literal_eqb l l' then True else False
+  | VCons hd tl, VCons hd' tl' => Vrel_rec n Vrel hd hd' /\ Vrel_rec n Vrel tl tl'
+  | VTuple l, VTuple l' =>
+    (fix go l l' :=
+      match l, l' with
+        | [], []        => True
+        | x::xs, y::ys  => Vrel_rec n Vrel x y /\ go xs ys
+        | _,  _         => False
+      end) l l'
+  | VMap l, VMap l' => True (*
+    (forall i, i < length l ->
+    Vrel_rec n Vrel Excrel (fst (nth i l (VNil, VNil))) (fst (nth i l' (VNil, VNil))) /\
+    Vrel_rec n Vrel Excrel (snd (nth i l (VNil, VNil))) (snd (nth i l' (VNil, VNil)))) *)
+  (* 
+  | EFun vl1 b1, EFun vl2 b2 =>
+    if length vl1 =? length vl2 then
+     forall m (Hmn : m < n), forall (vals1 vals2 : list Exp),
+       length vals1 = length vl1 -> length vals2 = length vl2 ->
+       list_biforall (Vrel m Hmn) vals1 vals2 
+     ->
+       exp_rel m (fun m' H => Vrel m' (Nat.le_lt_trans _ _ _ H Hmn)) 
+                 (b1.[list_subst (EFun vl1 b1 :: vals1) idsubst])
+                 (b2.[list_subst (EFun vl2 b2 :: vals2) idsubst])
+     else False
+  *)
+  
+  | VClos ext id vc e, VClos ext' id' vc' e' =>
+    vc = vc' /\
+    (forall m (Hmn : m < n),
+     forall (vl1 vl2 : list ValueExpression),
+     length vl1 = vc -> length vl2 = vc ->
+     Vrel m Hmn vl1 vl2 ->
+     exp_rel m (fun m' H => Vrel m' (Nat.le_lt_trans _ _ _ H Hmn))
+                (Excrel_rec m (fun m' H => Vrel m' (Nat.le_trans _ _ _ H Hmn)))
+                (e.[list_subst ((convert_to_closlist ext)++vl1) idsubst])
+                (e'.[list_subst ((convert_to_closlist ext')++vl2) idsubst])
+   )
+  | _, _ => False
+  end
+.
+*)
+
+
+Fixpoint Vrel_rec  (n : nat)
+                    (Vrel : forall m, m < n -> ValueExpression -> ValueExpression -> Prop)
+                    (v1 v2 : ValueExpression) : Prop :=
+  VALCLOSED v1 /\ VALCLOSED v2 /\
+  match v1, v2 with
+  | VNil, VNil => True
+  | VLit l, VLit l' => if Equalities.Literal_eqb l l' then True else False
+  | VCons hd tl, VCons hd' tl' => Vrel_rec n Vrel hd hd' /\ Vrel_rec n Vrel tl tl'
+  | VTuple l, VTuple l' =>
+    (fix go l l' :=
+      match l, l' with
+        | [], []        => True
+        | x::xs, y::ys  => Vrel_rec n Vrel x y /\ go xs ys
+        | _,  _         => False
+      end) l l'
+  | VMap l, VMap l' => 
+    (fix go l l' :=
+      match l, l' with
+        | [], []        => True
+        | (x1,x2)::xs, (y1,y2)::ys  => Vrel_rec n Vrel x1 y1 /\ Vrel_rec n Vrel x2 y2 /\ go xs ys
+        | _,  _         => False
+      end) l l'
+    (*
+    (forall i, i < length l ->
+    Vrel_rec n Vrel Excrel (fst (nth i l (VNil, VNil))) (fst (nth i l' (VNil, VNil))) /\
+    Vrel_rec n Vrel Excrel (snd (nth i l (VNil, VNil))) (snd (nth i l' (VNil, VNil)))) *)
+  
+  | VClos ext id vc e, VClos ext' id' vc' e' =>
+    vc = vc' /\
+    (forall m (Hmn : m < n),
+     forall (vl1 vl2 : list ValueExpression),
+     length vl1 = vc -> length vl2 = vc ->
+     list_biforall (Vrel m Hmn) vl1 vl2 ->
+     exp_rel m (fun m' H => Vrel m' (Nat.le_lt_trans _ _ _ H Hmn))
+                (e.[list_subst ((convert_to_closlist ext)++vl1) idsubst])
+                (e'.[list_subst ((convert_to_closlist ext')++vl2) idsubst])
+   )
+  | _, _ => False
+  end
+.
+
+Definition Vrel : nat -> ValueExpression -> ValueExpression -> Prop :=
+  Fix Wf_nat.lt_wf _ Vrel_rec.
+
+Definition Erel (n : nat) (e1 e2 : Expression) : Prop :=
+  exp_rel n (fun m _ => Vrel m) e1 e2.
+
+Definition Frel (n : nat) (K1 K2 : FrameStack) : Prop :=
+  frame_rel n (fun m _ => Vrel m) K1 K2.
+
+Definition Excrel (n: nat) (ex1 ex2 : Exception) : Prop :=
+  exc_rel n (fun m _ => Vrel m) ex1 ex2.
+
+
+(** ξ and η assigns closed expressions to vars in Γ 
+  Basically this says, ξ and η are equivalent pointwise for Γ
+*)
+
+Lemma Vrel_rec_pointwise {n : nat} :
+  forall (f g : forall m : nat, (m < n)%nat -> Exp -> Exp -> Prop),
+    (forall (m : nat) (p : (m < n)%nat), f m p = g m p) ->
+    Vrel_rec n f = Vrel_rec n g.
+Proof.
+  intros.
+  unfold Vrel_rec.
+  extensionality v1.
+  extensionality v2. generalize dependent v2.
+  induction v1; try destruct v2; intros; auto.
+  f_equal. f_equal.
+
+  cbn. break_match_goal. 2: auto.
+  
+  f_equal. f_equal.
+  extensionality m.
+  extensionality Hmn.
+  extensionality v1'.
+  extensionality v2'.
+  rewrite H.
+  extensionality l1. extensionality l2.
+  extensionality bif.
+  f_equal.
+  extensionality m'.
+  extensionality H0.
+  trivial.
+
+  do 2 f_equal.
+  rewrite IHv1_1, IHv1_2; auto.
+Qed.
+
+Lemma Vrel_Fix_eq : forall {n : nat} {v1 v2 : Exp},
+  Vrel n v1 v2
+  = 
+  Vrel_rec n (fun (m : nat) (_ : m < n) => Vrel m) v1 v2.
+Proof.
+  intros.
+  unfold Vrel.
+  rewrite Fix_eq by (auto using Vrel_rec_pointwise).
+  trivial.
+Qed.
+
+Definition inf := EApp (EFun [] (EApp (EFunId 0) [])) [].
+
+Theorem inf_diverges :
+  forall n Fs, ~|Fs, inf| n↓.
+Proof.
+  unfold inf.
+  intros. intro. induction n using lt_wf_ind. inversion H; try inversion_is_value. subst.
+  inversion H5; subst.
+  clear H5 H. simpl in H3.
+  eapply H0. 2: exact H3. lia.
+Qed.
+
+Scheme le_dep_ind := Induction for le Sort Prop.
+
+Lemma Vrel_downclosed :
+  forall {n m : nat} {Hmn : m <= n} {v1 v2 : Exp},
+    Vrel n v1 v2 ->
+    Vrel m v1 v2.
+Proof.
+  induction 1 using le_dep_ind;
+    intros;
+    eauto.
+  generalize dependent v2.
+  induction v1; destruct v2; intros; intuition; try break_match_hyp; intros.
+  rewrite Vrel_Fix_eq.
+  rewrite Vrel_Fix_eq in H.
+  unfold Vrel_rec at 1.
+  unfold Vrel_rec at 1 in H. intuition.
+
+  try break_match_hyp; intros. 2: contradiction.
+  simpl.
+  epose proof (H2 m1 _ vals1 vals2 H1 H3 H4). apply H5; auto.
+
+  rewrite Vrel_Fix_eq.
+  rewrite Vrel_Fix_eq in H. destruct H as [cl1 [cl2 H]].
+  split. 2: split. 1-2: auto.
+  simpl. simpl in H. intros.
+  specialize (IHv1_1 v2_1). specialize (IHv1_2 v2_2).
+  do 2 rewrite Vrel_Fix_eq in IHv1_1. do 2 rewrite Vrel_Fix_eq in IHv1_2.
+  split. apply IHv1_1, H. apply IHv1_2, H.
+Unshelve. lia.
+Qed.
+
+Lemma Erel_downclosed :
+  forall {n m : nat} {Hmn : m <= n} {e1 e2 : Exp},
+    Erel n e1 e2 ->
+    Erel m e1 e2.
+Proof.
+  intros.
+  unfold Erel, exp_rel.
+  unfold Erel, exp_rel in H.
+  destruct H, H0. split; auto. split; auto.
+  intros. eapply (H1 m0); eauto. lia.
+Qed.
+
+Lemma Vrel_closed : forall {n : nat} {v1 v2 : Exp},
+    Vrel n v1 v2 ->
+    VALCLOSED v1 /\ VALCLOSED v2.
+Proof.
+  intros. rewrite Vrel_Fix_eq in H.
+  Search "pointwise" "Vrel".
+  destruct v1, v2; destruct H as [Cl1 [Cl2 H]]; try inversion_is_value;
+  split; try contradiction.
+  all: auto.
+Qed.
+
+Lemma Vrel_closed_l : forall {n : nat} {v1 v2 : Exp},
+    Vrel n v1 v2 ->
+    VALCLOSED v1.
+Proof.
+  intros.
+  apply Vrel_closed in H.
+  intuition.
+Qed.
+
+Global Hint Resolve Vrel_closed_l : core.
+
+Lemma Vrel_closed_r : forall {n : nat} {v1 v2 : Exp},
+    Vrel n v1 v2 ->
+    VALCLOSED v2.
+Proof.
+  intros.
+  apply Vrel_closed in H.
+  intuition.
+Qed.
+
+Global Hint Resolve Vrel_closed_r : core.
+
+Lemma Erel_closed : forall {n : nat} {e1 e2 : Exp},
+    Erel n e1 e2 ->
+    EXPCLOSED e1 /\ EXPCLOSED e2.
+Proof.
+  intros.
+  unfold Erel, exp_rel in H.
+  intuition.
+Qed.
+
+Lemma Erel_closed_l : forall {n : nat} {e1 e2 : Exp},
+    Erel n e1 e2 ->
+    EXPCLOSED e1.
+Proof.
+  intros.
+  apply Erel_closed in H.
+  intuition.
+Qed.
+
+Global Hint Resolve Erel_closed_l : core.
+
+Lemma Erel_closed_r : forall {n : nat} {e1 e2 : Exp},
+    Erel n e1 e2 ->
+    EXPCLOSED e2.
+Proof.
+  intros.
+  apply Erel_closed in H.
+  intuition.
+Qed.
+
+Global Hint Resolve Erel_closed_r : core.
+
+
+(** closing substitutions *)
+Definition Grel (n : nat) (Γ : nat) (ξ₁ ξ₂ : Substitution) : Prop :=
+  SUBSCOPE Γ ⊢ ξ₁ ∷ 0 /\ SUBSCOPE Γ ⊢ ξ₂ ∷ 0 /\
+  forall x, x < Γ -> 
+    match (ξ₁ x), (ξ₂ x) with
+    | inl e1, inl e2 => Vrel n e1 e2
+    | _, _ => False
+    end.
+
+Lemma Grel_downclosed_helper : forall vals1 vals2 m n,
+  m <= n -> length vals1 = length vals2 ->
+  list_biforall (Vrel n) vals1 vals2 ->
+  list_biforall (Vrel m) vals1 vals2.
+Proof.
+  intro. induction vals1 using list_length_ind; intros.
+  destruct vals1, vals2.
+  * constructor.
+  * inversion H1.
+  * inversion H1.
+  * inversion H2. subst. constructor. 
+    - eapply Vrel_downclosed. eauto.
+    - eapply H; eauto.
+Unshelve. auto.
+Qed.
+
+Lemma Grel_downclosed :
+  forall {n m : nat} {Hmn : m <= n} {Γ : nat} {ξ₁ ξ₂ : Substitution},
+    Grel n Γ ξ₁ ξ₂ ->
+    Grel m Γ ξ₁ ξ₂ .
+Proof.
+  unfold Grel; intros.
+  unfold Grel; intros. intuition.
+  repeat break_match_goal; specialize (H2 x H1); try rewrite Heqs in H2; try rewrite Heqs0 in H2; [ intuition (eauto using Vrel_downclosed) | contradiction | contradiction ].
+Qed.
+
+Definition Vrel_open (Γ : nat) (e1 e2 : Exp) :=
+  forall n ξ₁ ξ₂,
+  Grel n Γ ξ₁ ξ₂
+->
+  Vrel n (subst ξ₁ e1) (subst ξ₂ e2).
+
+Definition Erel_open (Γ : nat) (e1 e2 : Exp) :=
+  forall n ξ₁ ξ₂,
+  Grel n Γ ξ₁ ξ₂
+->
+  Erel n (subst ξ₁ e1) (subst ξ₂ e2).
+
+Lemma Erel_open_closed : forall {Γ e1 e2},
+    Erel_open Γ e1 e2 ->
+    forall ξ, SUBSCOPE Γ ⊢ ξ ∷ 0 ->
+              EXPCLOSED (subst ξ e1) /\ EXPCLOSED (subst ξ e2).
+Proof.
+  intros.
+  apply @Erel_closed with (n:=0).
+  apply H; auto.
+  unfold Grel.
+  intuition idtac. break_match_goal.
+  (* rewrite Vrel_Fix_eq. unfold Vrel_rec at 1. *)
+  specialize (H0 x H1) as P'. rewrite Heqs in P'. clear dependent ξ.
+  * rewrite Vrel_Fix_eq. unfold Vrel_rec at 1.
+    induction e; intros; try inversion_is_value; auto; try lia.
+    constructor; auto. constructor; auto.
+    break_match_goal; intros; try congruence; try inversion Hmn.
+    rewrite Nat.eqb_refl in Heqb; congruence.
+
+    split. 2: split. auto. auto. intros. inversion P'. subst.
+    split. eapply IHe1; auto. eapply IHe2; auto.
+  * specialize (H0 x H1). rewrite Heqs in H0. lia.
+Qed.
+
+Lemma Erel_open_scope : forall {Γ e1 e2},
+    Erel_open Γ e1 e2 ->
+    EXP Γ ⊢ e1 /\ EXP Γ ⊢ e2.
+Proof.
+  intros.
+  pose proof (Erel_open_closed H).
+  split;
+  eapply (subst_implies_scope_exp); intros; apply H0; auto.
+Qed.
+
+Lemma Erel_open_scope_l : forall {Γ e1 e2},
+    Erel_open Γ e1 e2 ->
+    EXP Γ ⊢ e1.
+Proof.
+  intros. eapply Erel_open_scope in H. destruct H. auto.
+Qed.
+
+Global Hint Resolve Erel_open_scope_l : core.
+
+Lemma Erel_open_scope_r : forall {Γ e1 e2},
+    Erel_open Γ e1 e2 ->
+    EXP Γ ⊢ e2.
+Proof.
+  intros. eapply Erel_open_scope in H. destruct H. auto.
+Qed.
+
+Global Hint Resolve Erel_open_scope_r : core.
+
+Lemma Vrel_possibilities : forall {n v1 v2},
+  Vrel n v1 v2 ->
+  (exists n, v1 = ELit n /\ v2 = ELit n) \/
+  (exists p, v1 = EPid p /\ v2 = EPid p) \/
+  (exists vl1 vl2 b1 b2, v1 = EFun vl1 b1 /\ v2 = EFun vl2 b2) \/
+  (exists v11 v12 v21 v22, v1 = VCons v11 v12 /\ v2 = VCons v21 v22) \/
+  (v1 = ENil /\ v2 = ENil).
+Proof.
+  intros; destruct v1, v2; destruct H as [? [? ?] ]; subst; try contradiction.
+  * left. eexists; split. reflexivity. reflexivity.
+  * right. left. eexists; split. reflexivity. reflexivity.
+  * right. right. left. repeat eexists.
+  * intuition.
+  * right. right. right. left. repeat eexists.
+Qed.
+
+Lemma Vrel_open_closed : forall {Γ e1 e2},
+    Vrel_open Γ e1 e2 ->
+    forall ξ, SUBSCOPE Γ ⊢ ξ ∷ 0 ->
+              VALCLOSED (subst ξ e1) /\ VALCLOSED (subst ξ e2).
+Proof.
+  intros.
+  apply @Vrel_closed with (n:=0).
+  apply H; auto.
+  unfold Grel.
+  intuition idtac. break_match_goal.
+  specialize (H0 x H1) as P'. rewrite Heqs in P'.
+  rewrite Vrel_Fix_eq. clear dependent ξ.
+  induction e; intros; try congruence; try inversion Hmn;
+    try inversion_is_value; try lia.
+  1-4: split;[auto|split; auto].
+  * break_match_goal; intros; try congruence; try lia.
+    rewrite Nat.eqb_refl in Heqb; congruence.
+  * inversion P'. split; auto.
+  * epose proof (H0 x H1). rewrite Heqs in H2. lia.
+Qed.
+
+Lemma Vrel_open_scope : forall {Γ e1 e2},
+    Vrel_open Γ e1 e2 ->
+    VAL Γ ⊢ e1 /\ VAL Γ ⊢ e2.
+Proof.
+  intros.
+  pose proof (Vrel_open_closed H).
+  split;
+  eapply (subst_implies_scope_val); intros; apply H0; auto.
+Qed.
+
+Lemma Vrel_open_scope_l : forall {Γ e1 e2},
+    Vrel_open Γ e1 e2 ->
+    VAL Γ ⊢ e1.
+Proof.
+  intros. eapply Vrel_open_scope in H. destruct H. auto.
+Qed.
+
+Global Hint Resolve Vrel_open_scope_l : core.
+
+Lemma Vrel_open_scope_r : forall {Γ e1 e2},
+    Vrel_open Γ e1 e2 ->
+    VAL Γ ⊢ e2.
+Proof.
+  intros. eapply Vrel_open_scope in H. destruct H. auto.
+Qed.
+
+Global Hint Resolve Vrel_open_scope_r : core.
+
+Lemma Frel_downclosed :
+  forall {n m : nat} {Hmn : m <= n} {F1 F2 : FrameStack},
+    Frel n F1 F2 ->
+    Frel m F1 F2.
+Proof.
+  unfold Frel, frame_rel.
+  intuition. eapply H2 in H3. exact H3. lia. auto.
+Qed.
+
+Global Hint Resolve Frel_downclosed : core.
+
+Lemma Frel_closed : forall {n : nat} {F1 F2 : FrameStack},
+    Frel n F1 F2 ->
+    FSCLOSED F1 /\ FSCLOSED F2.
+Proof.
+  intros.
+  unfold Frel, frame_rel in H.
+  intuition.
+Qed.
+
+Lemma Frel_closed_l : forall {n : nat} {F1 F2 : FrameStack},
+    Frel n F1 F2 ->
+    FSCLOSED F1.
+Proof.
+  intros.
+  apply Frel_closed in H.
+  intuition.
+Qed.
+
+Global Hint Resolve Frel_closed_l : core.
+
+Lemma Frel_closed_r : forall {n : nat} {F1 F2 : FrameStack},
+    Frel n F1 F2 ->
+    FSCLOSED F2.
+Proof.
+  intros.
+  apply Frel_closed in H.
+  intuition.
+Qed.
+
+Global Hint Resolve Frel_closed_r : core.
+
+
+Lemma biforall_vrel_scoped : forall vals1 vals2 Γ,
+  list_biforall (Vrel_open Γ) vals1 vals2 ->
+  Forall (fun e => VAL Γ ⊢ e) vals1 /\ Forall (fun e => VAL Γ ⊢ e) vals2.
+Proof.
+  induction vals1; intros; inversion H; subst; repeat constructor.
+  * eapply Vrel_open_scope_l; eauto.
+  * specialize (IHvals1 _ _ H4); apply IHvals1.
+  * eapply Vrel_open_scope_r; eauto.
+  * eapply IHvals1; eauto.
+Qed.
+
+Lemma biforall_erel_scoped : forall vals1 vals2 Γ,
+  list_biforall (Erel_open Γ) vals1 vals2 ->
+  Forall (fun e => EXP Γ ⊢ e) vals1 /\ Forall (fun e => EXP Γ ⊢ e) vals2.
+Proof.
+  induction vals1; intros; inversion H; subst; split; constructor.
+  * eapply Erel_open_scope_l; eauto.
+  * specialize (IHvals1 _ _ H4); apply IHvals1.
+  * eapply Erel_open_scope_r; eauto.
+  * eapply IHvals1; eauto.
+Qed.
+
+Lemma biforall_vrel_closed : forall vals1 vals2 m,
+  list_biforall (Vrel m) vals1 vals2 ->
+  Forall (fun e => VALCLOSED e) vals1 /\ Forall (fun e => VALCLOSED e) vals2.
+Proof.
+  induction vals1; intros; inversion H; subst; repeat constructor.
+  * eapply Vrel_closed_l; eauto.
+  * specialize (IHvals1 _ _ H4); apply IHvals1.
+  * eapply Vrel_closed_r; eauto.
+  * eapply IHvals1; eauto.
+Qed.
+
+Lemma biforall_erel_closed : forall vals1 vals2 m,
+  list_biforall (Erel m) vals1 vals2 ->
+  Forall (fun e => EXPCLOSED e) vals1 /\ Forall (fun e => EXPCLOSED e) vals2.
+Proof.
+  induction vals1; intros; inversion H; subst; split; constructor.
+  * eapply Erel_closed_l; eauto.
+  * specialize (IHvals1 _ _ H4); apply IHvals1.
+  * eapply Erel_closed_r; eauto.
+  * eapply IHvals1; eauto.
+Qed.
+
+Lemma Grel_scons : forall n v1 v2 ξ₁ ξ₂ Γ,
+  Grel n Γ ξ₁ ξ₂ -> Vrel n v1 v2 -> Grel n (S Γ) (v1.:ξ₁) (v2.:ξ₂).
+Proof.
+  intros. split. 2: split.
+  1-2: apply cons_scope; auto.
+  2, 4: apply H. 1-2: now apply Vrel_closed in H0.
+  intros. destruct x; simpl; auto.
+  apply H. lia.
+Qed.
+
+Corollary Grel_list : forall n vl1 vl2 ξ₁ ξ₂ Γ,
+  Grel n Γ ξ₁ ξ₂ -> list_biforall (Vrel n) vl1 vl2 ->
+  Grel n (length vl1 + Γ) (list_subst vl1 ξ₁) (list_subst vl2 ξ₂).
+Proof.
+  induction vl1; intros; inversion H0; subst; simpl; auto.
+  apply Grel_scons; auto.
+Qed.
